fixing atomic spec machinery

atomics/verif_lock_atomic.v
@@ -46,11 +46,6 @@ Section PROOFS.
      LOCAL ()
      SEP ().
 
-(*Ltac atomic_nonexpansive_tac := try (let x := fresh "x" in intros ???? x;
-  repeat destruct x as [x ?]; solve_proper); try solve_proper.
-
-Obligation Tactic := try solve_proper.*)
-
   Program Definition release_spec :=
     DECLARE _release
     ATOMIC TYPE (ConstType val) INVS empty
@@ -66,7 +61,7 @@ Obligation Tactic := try solve_proper.*)
 
   Program Definition acquire_spec :=
     DECLARE _acquire
-    ATOMIC TYPE (ConstType _) OBJ l INVS empty
+    ATOMIC TYPE (ConstType val) OBJ l INVS empty
     WITH p
     PRE [ tptr t_lock ]
        PROP ()
@@ -114,7 +109,7 @@ Obligation Tactic := try solve_proper.*)
       + iApply atomic_int_at__. iAssumption.
       + iIntros "AA".
         iApply "H"; iFrame.
-    - entailer !.
+    - entailer!.
   Qed.
 
   Lemma body_acquire: semax_body Vprog Gprog f_acquire acquire_spec.
@@ -157,17 +152,17 @@ Obligation Tactic := try solve_proper.*)
 
   Lemma release_nonatomic: funspec_sub (snd release_spec) release_spec_nonatomic.
   Proof.
-    split; auto. intros. simpl in *. Intros.
-    unfold rev_curry, tcurry; simpl. iIntros "H !>". iExists (x2, atomic_int_at Ews (vint 0) x2), emp.
+    split; first done. intros p ?. simpl in *. Intros.
+    unfold rev_curry, tcurry; simpl. iIntros "H !>". iExists (p, atomic_int_at Ews (vint 0) p), emp.
     rewrite bi.emp_sep. iSplit.
-    - unfold PROPx, PARAMSx, GLOBALSx, LOCALx, SEPx, argsassert2assert; simpl.
+    - unfold PROPx, PARAMSx, GLOBALSx, LOCALx, SEPx, argsassert2assert; simpl; monPred.unseal.
       iDestruct "H" as "(% & % & _ & H & _)".
       do 4 (iSplit; auto).
       unfold atomic_shift; iAuIntro; unfold atomic_acc; simpl.
       iExists tt; iFrame "H".
       iApply fupd_mask_intro; first done; iIntros "Hclose".
       iSplit; [iIntros "$" | iIntros (_) "[$ _]"]; auto.
-    - iPureIntro. intros. Intros. rewrite emp_sepcon. auto.
+    - iPureIntro. intros. Intros. rewrite bi.emp_sep //.
   Qed.
 
 
@@ -177,68 +172,7 @@ Obligation Tactic := try solve_proper.*)
      we would be able to prove lock_specs directly (without using funspec_sub), but
      that conflicts with the "one spec in Gprog" approach. *)
 
-  #[local] Obligation Tactic := intros.
-
-  #[export] Program Instance atomic_impl : lock_impl := { t_lock := Tstruct _atom_int noattr; lock_handle := val * namespace * ghosts.gname;
-    ptr_of h := let '(v, _, _) := h in v; lock_inv sh h R := let '(v, N, g) := h in !!(sh <> Share.bot /\ isptr v) && cinv N g (inv_for_lock v R) * cinv_own g sh }.
-  Next Obligation.
-  Proof.
-    destruct h as ((?, ?), ?).
-    apply sepcon_nonexpansive, const_nonexpansive.
-    apply @conj_nonexpansive; [apply const_nonexpansive|].
-    apply cinv_nonexpansive2, inv_for_lock_nonexpansive.
-  Qed.
-  Next Obligation.
-  Proof.
-    destruct h as ((?, ?), ?); simpl.
-    destruct (isptr_dec v).
-    rewrite !prop_true_andp; auto.
-    rewrite <- !sepcon_assoc, (sepcon_comm (_ * cinv_own _ _)), !sepcon_assoc.
-    unfold cinv_own at 1 2; erewrite <- own_op by eauto.
-    rewrite <- sepcon_assoc; f_equal.
-    rewrite {3}(bi.persistent_sep_dup (cinv n g _)); auto.
-    { split; auto; intros ?; subst. apply join_Bot in H1 as []; contradiction. }
-    { rewrite -> prop_false_andp, !FF_sepcon, prop_false_andp, FF_sepcon; auto; intros []; contradiction. }
-  Qed.
-  Next Obligation.
-  Proof.
-    unfold exclusive_mpred; destruct h as ((?, ?), ?); Intros.
-    unfold cinv_own; sep_apply own_op'.
-    Intros ?; Intros.
-    apply sepalg.join_self, identity_share_bot in H0; contradiction.
-  Qed.
-  Next Obligation.
-  Proof.
-    destruct h as ((?, ?), ?); simpl; entailer!.
-  Qed.
-
-  Definition name_of (h : lock_handle) := let '(_, N, _) := h in N.
-  Definition ghost_of (h : lock_handle) := let '(_, _, g) := h in g.
-  #[global] Instance lock_handle_inhabited : Inhabitant lock_handle := (Vundef, nroot, O).
-
-  (* Since a lock's namespace is known, the ghost name is the only part that needs to be existentially quantified. *)
-  Definition self_part sh h := cinv_own (ghost_of h) sh.
-
-  Lemma self_part_exclusive : forall sh h, sh <> Share.bot -> exclusive_mpred (self_part sh h).
-  Proof.
-    intros; unfold exclusive_mpred, self_part.
-    unfold cinv_own; rewrite own_op'; Intros ?.
-    apply sepalg.join_self, identity_share_bot in H0; contradiction.
-  Qed.
-
-  Lemma self_part_eq : forall sh1 sh2 h R, sh2 <> Share.bot -> lock_inv sh1 h (self_part sh2 h * R) * self_part sh2 h =
-    lock_inv sh1 h (self_part sh2 h * R) * lock_inv sh2 h (self_part sh2 h * R).
-  Proof.
-    intros; unfold lock_inv; destruct h as ((v, N), g); simpl.
-    destruct (eq_dec sh1 Share.bot).
-    { rewrite -> prop_false_andp, !FF_sepcon; auto; intros []; contradiction. }
-    destruct (isptr_dec v).
-    rewrite -> !prop_true_andp by auto.
-    unfold self_part at 2; rewrite {1}(bi.persistent_sep_dup (cinv N g _)).
-    rewrite <- !sepcon_assoc; f_equal.
-    rewrite -> (sepcon_comm (_ * _) (cinv _ _ _)), <- sepcon_assoc; reflexivity.
-    { rewrite -> prop_false_andp, !FF_sepcon; auto; intros []; contradiction. }
-  Qed.
+  Definition name_of (h : lock_handle) := let '(v, i, g) := h in i.
 
   (* caller can request the lock's namespace *)
   Program Definition makelock_spec_inv :=
@@ -250,96 +184,67 @@ Obligation Tactic := try solve_proper.*)
     POST [ tptr t_lock ] (* asymmetric consequence makes this messy *) ∃ v,
        PROP ()
        RETURN (v)
-       SEP (mem_mgr gv; |={⊤}=> ∃ h, !!(ptr_of h = v /\ name_of h = N) && lock_inv Tsh h (R h)).
-  Next Obligation.
-  Proof.
-    repeat intro.
-    destruct x as ((?, ?), ?); simpl.
-    reflexivity.
-  Qed.
-  Next Obligation.
-  Proof.
-    repeat intro.
-    destruct x as ((?, ?), ?); simpl.
-    rewrite -> 2approx_exp; apply f_equal; extensionality.
-    unfold PROPx, PARAMSx, GLOBALSx, LOCALx, SEPx, argsassert2assert; simpl; rewrite -> !approx_andp; do 2 apply f_equal;
-      rewrite -> !sepcon_emp, ?approx_sepcon, ?approx_idem.
-    apply f_equal. setoid_rewrite fupd_nonexpansive; do 2 apply f_equal.
-    rewrite !approx_exp; apply f_equal; extensionality.
-    rewrite !approx_andp; f_equal.
-    apply lock_inv_super_non_expansive.
-  Qed.
+       SEP (mem_mgr gv; |={⊤}=> ∃ h, ⌜ptr_of h = v /\ name_of h = N⌝ ∧ lock_inv 1 h (R h)).
 
   (* These lemmas can be used to attach an invariant to an existing lock. *)
-  Lemma make_lock_inv_1 : forall v N (R : lock_handle -> mpred), atomic_int_at Ews (vint 1) v |-- (*|={⊤}=>*) @fupd mpred (bi_fupd_fupd(BiFUpd := mpred_bi_fupd)) ⊤ ⊤ (∃ h, !!(ptr_of h = v /\ name_of h = N) && lock_inv Tsh h (R h)).
+  Lemma make_lock_inv_1 : forall v N (R : lock_handle -> mpred), atomic_int_at Ews (vint 1) v ⊢ |={⊤}=> (∃ h, ⌜ptr_of h = v /\ name_of h = N⌝ ∧ lock_inv 1 h (R h)).
   Proof.
     intros.
     iIntros "a".
     iDestruct (atomic_int_isptr with "a") as %Ha.
-    iMod (cinv_alloc_dep with "[a]") as (g) "[Hi Hg]";
-      [| iExists (v, N, g); unfold lock_inv; simpl; iFrame "Hi Hg"; auto].
-    iIntros (?) "!>"; unfold inv_for_lock.
-    iExists true; iFrame.
+    iMod cinv_alloc_strong as (g) "(_ & Hg & Hi)"; first apply pred_infinite_True.
+    iExists (v, N, g); unfold lock_inv; simpl; iFrame.
+    iMod ("Hi" $! (inv_for_lock v (R (v, N, g))) with "[-]").
+    { iExists true; iFrame; done. }
+    iFrame; done.
   Qed.
 
-  Lemma make_lock_inv_0_self : forall v N R sh1 sh2, sh1 <> Share.bot -> sepalg.join sh1 sh2 Tsh ->
-    (atomic_int_at Ews (vint 0) v * R) |-- @fupd mpred (bi_fupd_fupd(BiFUpd := mpred_bi_fupd)) ⊤ ⊤ (∃ h, !!(ptr_of h = v /\ name_of h = N) && lock_inv sh1 h (R * self_part sh2 h)).
+  Lemma make_lock_inv_0_self : forall v N R sh1 sh2, sh1 ⋅ sh2 = 1%Qp ->
+    (atomic_int_at Ews (vint 0) v ∗ R) ⊢ |={⊤}=> (∃ h, ⌜ptr_of h = v /\ name_of h = N⌝ ∧ lock_inv sh1 h (R ∗ self_part sh2 h)).
   Proof.
     intros.
     iIntros "[a R]".
     iDestruct (atomic_int_isptr with "a") as %Ha.
-    iMod (own_alloc(RA := share_ghost) with "[$]") as (g) "g"; first done.
-    setoid_rewrite (own_op(RA := share_ghost) _ _ _ _ _ H0); iDestruct "g" as "[g1 g2]".
-    iMod (inv_alloc with "[a R g2]") as "I";
-      [| iExists (v, N, g); unfold lock_inv; simpl; iFrame; auto].
-    iIntros "!>"; unfold inv_for_lock.
-    iLeft; iExists false; iFrame; auto.
+    iMod cinv_alloc_strong as (g) "(_ & Hg & Hi)"; first apply pred_infinite_True.
+    iExists (v, N, g); unfold lock_inv; simpl.
+    rewrite -H; iDestruct "Hg" as "($ & Hg)".
+    iMod ("Hi" $! (inv_for_lock v (R ∗ cinv_own g sh2)) with "[-]").
+    { iExists false; iFrame; done. }
+    iFrame; done.
   Qed.
 
-  Lemma make_lock_inv_0' : forall v N (R : lock_handle -> mpred), (atomic_int_at Ews (vint 0) v * ALL g, R g) |-- @fupd mpred (bi_fupd_fupd(BiFUpd := mpred_bi_fupd)) ⊤ ⊤ (∃ h, !!(ptr_of h = v /\ name_of h = N) && lock_inv Tsh h (R h)).
+  Lemma make_lock_inv_0' : forall v N (R : lock_handle -> mpred), (atomic_int_at Ews (vint 0) v ∗ ∀ g, R g) ⊢ |={⊤}=> (∃ h, ⌜ptr_of h = v /\ name_of h = N⌝ ∧ lock_inv 1 h (R h)).
   Proof.
     intros.
     iIntros "[a R]".
     iDestruct (atomic_int_isptr with "a") as %Ha.
-    iMod (cinv_alloc_dep with "[a R]") as (g) "[Hi Hg]";
-      [| iExists (v, N, g); unfold lock_inv; simpl; iFrame "Hi Hg"; auto].
-    iIntros (?) "!>"; unfold inv_for_lock.
-    iExists false; iFrame; auto.
+    iMod cinv_alloc_strong as (g) "(_ & Hg & Hi)"; first apply pred_infinite_True.
+    iExists (v, N, g); unfold lock_inv; simpl; iFrame.
+    iMod ("Hi" $! (inv_for_lock v (R (v, N, g))) with "[-]").
+    { iExists false; iFrame; done. }
+    iFrame; done.
   Qed.
 
-  Lemma make_lock_inv_0 : forall v N R, atomic_int_at Ews (vint 0) v * R |-- @fupd mpred (bi_fupd_fupd(BiFUpd := mpred_bi_fupd)) ⊤ ⊤ (∃ h, !!(ptr_of h = v /\ name_of h = N) && lock_inv Tsh h R).
+  Lemma make_lock_inv_0 : forall v N R, atomic_int_at Ews (vint 0) v ∗ R ⊢ |={⊤}=> (∃ h, ⌜ptr_of h = v /\ name_of h = N⌝ ∧ lock_inv 1 h R).
   Proof.
     intros.
-    eapply derives_trans, make_lock_inv_0'.
-    cancel.
-    apply allp_right; intros; auto.
+    rewrite -make_lock_inv_0'.
+    by iIntros "($ & $)".
   Qed.
 
   Lemma makelock_inv: funspec_sub (snd makelock_spec) makelock_spec_inv.
   Proof.
-    apply prove_funspec_sub.
-    split; auto. intros. simpl in *. destruct x2 as [[gv N] R]. Intros.
-    iIntros "H !>". iExists nil, gv, emp. rewrite emp_sepcon. iSplit; auto.
-    iPureIntro. intros. Intros. rewrite emp_sepcon. Intros x; Exists x.
-    unfold PROPx, PARAMSx, GLOBALSx, LOCALx, SEPx; simpl. Intros.
-    apply andp_right; [apply andp_left1, derives_refl | apply andp_left2].
-    cancel.
-    apply make_lock_inv_1.
+    split; first done. intros ((gv, N), R) ?; simpl in *. Intros.
+    iIntros "H !>". iExists gv, emp. rewrite bi.emp_sep. iSplit; auto.
+    iPureIntro. intros. Intros. rewrite bi.emp_sep. monPred.unseal. Intros x; Exists x.
+    iIntros "(? & $ & $ & ? & _)".
+    iSplit; first done.
+    rewrite bi.sep_emp; by iApply make_lock_inv_1.
   Qed.
-
-  #[local] Obligation Tactic := atomic_nonexpansive_tac.
-
-  Lemma inv_for_lock_super_non_expansive : forall p R n,
-    compcert_rmaps.RML.R.approx n (inv_for_lock p R) =
-    compcert_rmaps.RML.R.approx n (inv_for_lock p (compcert_rmaps.RML.R.approx n R)).
-  Proof.
-    intros; apply nonexpansive_super_non_expansive, inv_for_lock_nonexpansive.
-  Qed.
-  #[local] Hint Resolve inv_for_lock_super_non_expansive : core.
 
   (* Yet another variant: we only learn the lock invariant after a successful acquire. *)
   Program Definition acquire_spec_inv_atomic1 :=
-    ATOMIC TYPE (ConstType _) OBJ R INVS empty
+    ATOMIC TYPE (ConstType val) OBJ R INVS empty
     WITH p
     PRE [ tptr t_lock ]
        PROP ()
@@ -348,16 +253,15 @@ Obligation Tactic := try solve_proper.*)
     POST [ tvoid ]
        PROP ()
        LOCAL ()
-       SEP () | (inv_for_lock p R * R).
+       SEP () | (inv_for_lock p R ∗ R).
 
   Lemma acquire_inv_atomic: funspec_sub (snd acquire_spec) acquire_spec_inv_atomic1.
   Proof.
-    apply prove_funspec_sub.
-    split; auto. intros. simpl in *. destruct x2 as (p, Q). Intros.
-    unfold rev_curry, tcurry; simpl. iIntros "H !>". iExists nil.
+    split; first done. intros (p, Q) ?; simpl in *. Intros.
+    unfold rev_curry, tcurry; simpl. iIntros "H !>".
     iExists (p, Q), emp; simpl.
-    rewrite emp_sepcon. iSplit.
-    - unfold PROPx, PARAMSx, GLOBALSx, LOCALx, SEPx, argsassert2assert; simpl.
+    rewrite bi.emp_sep. iSplit.
+    - unfold PROPx, PARAMSx, GLOBALSx, LOCALx, SEPx, argsassert2assert; simpl; monPred.unseal.
       iDestruct "H" as "(% & % & _ & H & _)".
       do 4 (iSplit; auto).
       unfold atomic_shift; iAuIntro; unfold atomic_acc; simpl.
@@ -369,13 +273,13 @@ Obligation Tactic := try solve_proper.*)
         iExists b; iFrame.
       + iIntros (_) "[[% H1] _]"; subst.
         iDestruct "Hclose" as "[_ Hclose]"; iApply ("Hclose" $! tt).
-        rewrite sepcon_emp; iFrame "R"; iExists true; iFrame.
+        rewrite bi.sep_emp; iFrame "R"; iExists true; iFrame.
     - iPureIntro. iIntros (rho') "[% [_ H]]".
       unfold PROPx, LOCALx, SEPx; simpl; auto.
   Qed.
 
   Program Definition acquire_spec_inv_atomic :=
-    ATOMIC TYPE (ProdType (ConstType _) Mpred) INVS empty
+    ATOMIC TYPE (ProdType (ConstType val) Mpred) INVS empty
     WITH p, R
     PRE [ tptr t_lock ]
        PROP ()
@@ -385,23 +289,14 @@ Obligation Tactic := try solve_proper.*)
        PROP ()
        LOCAL ()
        SEP (R) | (inv_for_lock p R).
-  Next Obligation.
-  Proof.
-    intros; rewrite !approx_sepcon; f_equal; auto.
-  Qed.
-  Next Obligation.
-  Proof.
-    rewrite approx_idem; auto.
-  Qed.
 
   Lemma acquire_inv: funspec_sub (snd acquire_spec) acquire_spec_inv_atomic.
   Proof.
-    apply prove_funspec_sub.
-    split; auto. intros. simpl in *. destruct x2 as ((p, R), Q). Intros.
-    unfold rev_curry, tcurry; simpl. iIntros "H !>". iExists nil.
-    iExists (p, Q * R), emp; simpl.
-    rewrite emp_sepcon. iSplit.
-    - unfold PROPx, PARAMSx, GLOBALSx, LOCALx, SEPx, argsassert2assert; simpl.
+    split; first done. intros. simpl in *. destruct x2 as ((p, R), Q). Intros.
+    unfold rev_curry, tcurry; simpl. iIntros "H !>".
+    iExists (p, Q ∗ R), emp; simpl.
+    rewrite bi.emp_sep. iSplit.
+    - unfold PROPx, PARAMSx, GLOBALSx, LOCALx, SEPx, argsassert2assert; simpl; monPred.unseal.
       iDestruct "H" as "(% & % & _ & H & _)".
       do 4 (iSplit; auto).
       unfold atomic_shift; iAuIntro; unfold atomic_acc; simpl.
@@ -414,12 +309,12 @@ Obligation Tactic := try solve_proper.*)
       + iIntros (_) "[[% H1] _]"; subst.
         iFrame "R".
         iDestruct "Hclose" as "[_ Hclose]"; iApply ("Hclose" $! tt).
-        rewrite sepcon_emp; iExists true; iFrame.
+        rewrite bi.sep_emp; iExists true; iFrame.
     - iPureIntro. iIntros (rho') "[% [_ H]]".
-      unfold PROPx, LOCALx, SEPx; simpl. rewrite <- sepcon_assoc; auto.
+      unfold PROPx, LOCALx, SEPx; simpl. rewrite bi.sep_assoc //.
   Qed.
 
-  (* "lock variant" version where the lock has a parameter held in the global state *)
+(*  (* "lock variant" version where the lock has a parameter held in the global state *)
   Program Definition acquire_spec_inv_variant :=
     ATOMIC TYPE (ProdType (ConstType _) (ArrowType (DependentType 0) Mpred)) OBJ x INVS empty
     WITH p, R
@@ -443,7 +338,7 @@ Obligation Tactic := try solve_proper.*)
     split; auto. intros. simpl in *. destruct x2 as ((p, R), Q). Intros.
     unfold rev_curry, tcurry; simpl. iIntros "H !>". iExists nil.
     iExists (p, Q), emp; simpl.
-    rewrite emp_sepcon. iSplit.
+    rewrite bi.emp_sep. iSplit.
     - unfold PROPx, PARAMSx, GLOBALSx, LOCALx, SEPx, argsassert2assert; simpl.
       iDestruct "H" as "(% & % & _ & H & _)".
       do 4 (iSplit; auto).
@@ -456,46 +351,30 @@ Obligation Tactic := try solve_proper.*)
         iExists b; iFrame.
       + iIntros (_) "[[% H1] _]"; subst.
         iDestruct "Hclose" as "[_ Hclose]"; iApply ("Hclose" $! tt).
-        rewrite sepcon_emp; iFrame "R"; iExists true; iFrame.
+        rewrite bi.sep_emp; iFrame "R"; iExists true; iFrame.
     - iPureIntro. iIntros (rho') "[% [_ H]]".
       unfold PROPx, LOCALx, SEPx; simpl; auto.
-  Qed.
+  Qed.*)
 
   Program Definition release_spec_inv_atomic :=
-    ATOMIC TYPE (ProdType (ConstType _) Mpred) INVS empty
+    ATOMIC TYPE (ProdType (ConstType val) Mpred) INVS empty
     WITH p, R
     PRE [ tptr t_lock ]
        PROP ()
        PARAMS (p)
-       SEP (weak_exclusive_mpred R && emp) | (R * inv_for_lock p R)
+       SEP (<affine> (R ∗ R -∗ False)) | (R ∗ inv_for_lock p R)
     POST [ tvoid ]
        PROP ()
        LOCAL ()
        SEP () | (inv_for_lock p R).
-  Next Obligation.
-  Proof.
-    rewrite !approx_andp; f_equal.
-    apply nonexpansive_super_non_expansive, exclusive_mpred_nonexpansive.
-  Qed.
-  Next Obligation.
-  Proof.
-    intros; rewrite !approx_sepcon approx_idem; f_equal.
-    apply inv_for_lock_super_non_expansive.
-  Qed.
-  Next Obligation.
-  Proof.
-    intros; rewrite !approx_sepcon; f_equal.
-    apply inv_for_lock_super_non_expansive.
-  Qed.
 
   Lemma release_inv: funspec_sub (snd release_spec) release_spec_inv_atomic.
   Proof.
-    apply prove_funspec_sub.
-    split; auto. intros. simpl in *. destruct x2 as ((p, R), Q). Intros.
-    unfold rev_curry, tcurry; simpl. iIntros "H !>". iExists nil.
+    split; first done. intros ((p, R), Q) ?. simpl in *. Intros.
+    unfold rev_curry, tcurry; simpl. iIntros "H !>".
     iExists (p, Q), emp; simpl.
-    rewrite emp_sepcon. iSplit.
-    - unfold PROPx, PARAMSx, GLOBALSx, LOCALx, SEPx, argsassert2assert; simpl.
+    rewrite bi.emp_sep. iSplit.
+    - unfold PROPx, PARAMSx, GLOBALSx, LOCALx, SEPx, argsassert2assert; simpl; monPred.unseal.
       iDestruct "H" as "(% & % & _ & H & excl & _)".
       do 4 (iSplit; auto).
       unfold atomic_shift; iAuIntro; unfold atomic_acc; simpl.
@@ -509,20 +388,20 @@ Obligation Tactic := try solve_proper.*)
         * iIntros (_) "[H1 _]".
           iDestruct "excl" as "_".
           iDestruct "Hclose" as "[_ Hclose]"; iApply ("Hclose" $! tt).
-          rewrite sepcon_emp; iExists false; iFrame.
-      + iAssert (|> FF) with "[excl R R1]" as ">[]".
-        iNext. iApply weak_exclusive_conflict; iFrame; iFrame.
+          rewrite bi.sep_emp; iExists false; iFrame.
+      + iAssert (▷ False) with "[excl R R1]" as ">[]".
+        rewrite bi.affinely_elim; iApply "excl"; by iFrame.
     - iPureIntro. iIntros (rho') "[% [_ H]]".
       unfold PROPx, LOCALx, SEPx; simpl; auto.
   Qed.
 
   Program Definition release_spec_inv_atomic1 :=
-    ATOMIC TYPE (ConstType _) OBJ R INVS empty
+    ATOMIC TYPE (ConstType val) OBJ R INVS empty
     WITH p
     PRE [ tptr t_lock ]
        PROP ()
        PARAMS (p)
-       SEP () | ((weak_exclusive_mpred R && emp) * R * inv_for_lock p R)
+       SEP () | (<affine> (R ∗ R -∗ False) ∗ R ∗ inv_for_lock p R)
     POST [ tvoid ]
        PROP ()
        LOCAL ()
@@ -530,18 +409,17 @@ Obligation Tactic := try solve_proper.*)
 
   Lemma release_inv_atomic: funspec_sub (snd release_spec) release_spec_inv_atomic1.
   Proof.
-    apply prove_funspec_sub.
-    split; auto. intros. simpl in *. destruct x2 as (p, Q). Intros.
-    unfold rev_curry, tcurry; simpl. iIntros "H !>". iExists nil.
+    split; first done. intros (p, Q) ?. simpl in *. Intros.
+    unfold rev_curry, tcurry; simpl. iIntros "H !>".
     iExists (p, Q), emp; simpl.
-    rewrite emp_sepcon. iSplit.
-    - unfold PROPx, PARAMSx, GLOBALSx, LOCALx, SEPx, argsassert2assert; simpl.
+    rewrite bi.emp_sep. iSplit.
+    - unfold PROPx, PARAMSx, GLOBALSx, LOCALx, SEPx, argsassert2assert; simpl; monPred.unseal.
       iDestruct "H" as "(% & % & _ & H & _)".
       do 4 (iSplit; auto).
       unfold atomic_shift; iAuIntro; unfold atomic_acc; simpl.
       iMod "H" as (R) "[H Hclose]".
       unfold inv_for_lock at 1.
-      iDestruct "H" as "[[excl R] H1]"; iExists tt.
+      iDestruct "H" as "(excl & R & H1)"; iExists tt.
       iDestruct "H1" as (b) "[H1 R1]".
       destruct b.
       iFrame "H1".
@@ -550,83 +428,20 @@ Obligation Tactic := try solve_proper.*)
         iFrame "excl R"; iExists true; iFrame.
       + iIntros (_) "[H1 _]".
         iDestruct "Hclose" as "[_ Hclose]"; iApply ("Hclose" $! tt).
-        rewrite sepcon_emp; iExists false; iFrame.
-      + iAssert (|> FF) with "[excl R R1]" as ">[]".
-        iNext. iApply weak_exclusive_conflict; iFrame; iFrame.
+        rewrite bi.sep_emp; iExists false; iFrame.
+      + iAssert (▷ False) with "[excl R R1]" as ">[]".
+        rewrite bi.affinely_elim; iApply "excl"; by iFrame.
     - iPureIntro. iIntros (rho') "[% [_ H]]".
       unfold PROPx, LOCALx, SEPx; simpl; auto.
   Qed.
 
-  Definition exclusive_mpred' {A} (P : A -> mpred) := forall x y, P x * P y |-- FF.
-
-  Definition weak_exclusive_mpred' {A} (P : A -> mpred) := unfash (fash (ALL x y, P x * P y --> FF)).
-
-  Lemma approx_unfash_fash : forall n P, compcert_rmaps.RML.R.approx n (unfash (fash P)) = unfash (fash (compcert_rmaps.RML.R.approx n P)).
-  Proof.
-    intros; change unfash with subtypes.unfash; change fash with subtypes.fash; apply predicates_hered.pred_ext; intros ??.
-    - destruct H; intros ??; split; [lia | apply H0; auto].
-    - destruct (H a); auto; split; auto.
-      intros ??; apply H; auto.
-  Qed.
-
-  Lemma exclusive_mpred'_super_non_expansive:
-    forall {A} (R : A -> mpred) n, compcert_rmaps.RML.R.approx n (weak_exclusive_mpred' R) =
-      compcert_rmaps.RML.R.approx n (weak_exclusive_mpred' (fun a => compcert_rmaps.RML.R.approx n (R a))).
-  Proof.
-    intros; unfold weak_exclusive_mpred'.
-    rewrite !approx_unfash_fash; do 2 f_equal.
-    setoid_rewrite allp_nonexpansive; do 2 f_equal; extensionality.
-    setoid_rewrite allp_nonexpansive; do 2 f_equal; extensionality.
-    rewrite approx_imp; do 2 f_equal.
-    - apply approx_sepcon.
-    - apply approx_FF.
-  Qed.
-
-  Lemma fash_allp : forall {B} (F : B -> mpred), fash (allp F) = ALL x, fash (F x).
-  Proof.
-    intros; apply (subtypes.fash_allp B F).
-  Qed.
-
-  Lemma exclusive_weak_exclusive1' : forall {A} (R : A -> mpred) P,
-    exclusive_mpred' R ->
-    P |-- weak_exclusive_mpred' R.
-  Proof.
-    intros; unfold weak_exclusive_mpred'; unfold exclusive_mpred' in H.
-    rewrite fash_allp unfash_allp; apply allp_right; intros x.
-    rewrite fash_allp unfash_allp; apply allp_right; intros y.
-    specialize (H x y).
-    unseal_derives; apply derives_unfash_fash; auto.
-  Qed.
-
-  Lemma exclusive_weak_exclusive' : forall {A} (R : A -> mpred),
-    exclusive_mpred' R ->
-    seplog.emp |-- weak_exclusive_mpred' R && emp.
-  Proof.
-    intros; apply andp_right, derives_refl; apply exclusive_weak_exclusive1'; auto.
-  Qed.
-
-  Lemma corable_weak_exclusive' : forall {A} (R : A -> mpred), corable (weak_exclusive_mpred' R).
-  Proof.
-    intros; apply assert_lemmas.corable_unfash, _.
-  Qed.
-
-  Lemma weak_exclusive'_conflict : forall {A} P (x y : A),
-    (weak_exclusive_mpred' P && emp) * P x * P y |-- FF.
-  Proof.
-    intros.
-    rewrite sepcon_assoc -andp_left_corable; last by (apply corable_weak_exclusive').
-    unseal_derives; intros ? [].
-    unfold weak_exclusive_mpred in H; specialize (H a ltac:(lia) x y _ _ (ageable.necR_refl _) (predicates_hered.ext_refl _)).
-    apply H; auto.
-  Qed.
-
-  Program Definition release_spec_inv_variant :=
+(*  Program Definition release_spec_inv_variant :=
     ATOMIC TYPE (ProdType (ProdType (ConstType _) (ArrowType (DependentType 0) Mpred)) (DependentType 0)) OBJ y INVS empty
     WITH p, R, x
     PRE [ tptr t_lock ]
        PROP ()
        PARAMS (p)
-       SEP (weak_exclusive_mpred' R && emp) | (R x * inv_for_lock p (R y))
+       SEP (<affine> (R ∗ R -∗ False)) | (R x ∗ inv_for_lock p (R y))
     POST [ tvoid ]
        PROP ()
        LOCAL ()
@@ -653,7 +468,7 @@ Obligation Tactic := try solve_proper.*)
     split; auto. intros. simpl in *. destruct x2 as (((p, R), x), Q). Intros.
     unfold rev_curry, tcurry; simpl. iIntros "H !>". iExists nil.
     iExists (p, Q), emp; simpl.
-    rewrite emp_sepcon. iSplit.
+    rewrite bi.emp_sep. iSplit.
     - unfold PROPx, PARAMSx, GLOBALSx, LOCALx, SEPx, argsassert2assert; simpl.
       iDestruct "H" as "(% & % & _ & H & excl & _)".
       do 4 (iSplit; auto).
@@ -668,17 +483,15 @@ Obligation Tactic := try solve_proper.*)
         * iIntros (_) "[H1 _]".
           iDestruct "excl" as "_".
           iDestruct "Hclose" as "[_ Hclose]"; iApply ("Hclose" $! tt).
-          rewrite sepcon_emp; iExists false; iFrame.
-      + iAssert (|> FF) with "[excl R R1]" as ">[]".
+          rewrite bi.sep_emp; iExists false; iFrame.
+      + iAssert (▷ FF) with "[excl R R1]" as ">[]".
         iNext. iApply weak_exclusive'_conflict; iFrame; iFrame.
     - iPureIntro. iIntros (rho') "[% [_ H]]".
       unfold PROPx, LOCALx, SEPx; simpl; auto.
-  Qed.
-
-  #[local] Obligation Tactic := intros.
+  Qed.*)
 
   Program Definition acquire_spec_inv :=
-    TYPE (ProdType (ConstType _) Mpred)
+    TYPE (ProdType (ConstType (Qp * lock_handle)) Mpred)
     WITH sh : _, h : _, R : _
     PRE [ tptr t_lock ]
        PROP ()
@@ -687,33 +500,15 @@ Obligation Tactic := try solve_proper.*)
     POST [ tvoid ]
        PROP ()
        LOCAL ()
-       SEP (lock_inv sh h R; |> R).
-  Next Obligation.
-  Proof.
-    repeat intro.
-    destruct x as ((?, ?), ?); simpl.
-    unfold PROPx, PARAMSx, GLOBALSx, LOCALx, SEPx, argsassert2assert; simpl; rewrite !approx_andp; do 3 f_equal;
-      rewrite -> !sepcon_emp, ?approx_sepcon, ?approx_idem.
-    apply lock_inv_super_non_expansive.
-  Qed.
-  Next Obligation.
-  Proof.
-    repeat intro.
-    destruct x as ((?, ?), ?); simpl.
-    unfold PROPx, LOCALx, SEPx; simpl; rewrite !approx_andp; do 2 f_equal;
-      rewrite -> !sepcon_emp, ?approx_sepcon, ?approx_idem.
-    f_equal. apply lock_inv_super_non_expansive.
-    setoid_rewrite later_nonexpansive; rewrite approx_idem; auto.
-  Qed.
+       SEP (lock_inv sh h R; ▷ R).
 
   Lemma acquire_inv_simple: funspec_sub (snd acquire_spec) acquire_spec_inv.
   Proof.
-    apply prove_funspec_sub.
-    split; auto. intros. simpl in *. destruct x2 as ((sh, h), R). Intros.
-    unfold rev_curry, tcurry. iIntros "H !>". iExists nil.
-    iExists (@ptr_of atomic_impl h, @lock_inv atomic_impl sh h R * |> R), emp; simpl.
-    rewrite emp_sepcon. iSplit.
-    - unfold PROPx, PARAMSx, GLOBALSx, LOCALx, SEPx; simpl.
+    split; first done. intros ((sh, h), R) ?. simpl in *. Intros.
+    unfold rev_curry, tcurry. iIntros "H !>".
+    iExists (ptr_of(lock_impl := atomic_impl) h, lock_inv(lock_impl := atomic_impl) sh h R ∗ ▷ R), emp; simpl.
+    rewrite bi.emp_sep. iSplit.
+    - unfold PROPx, PARAMSx, GLOBALSx, LOCALx, SEPx; simpl; monPred.unseal.
       iDestruct "H" as "(_ & % & _ & H & _)".
       do 4 (iSplit; auto).
       unfold lock_inv; simpl; destruct h as ((v, i), g).
@@ -744,17 +539,17 @@ Obligation Tactic := try solve_proper.*)
     PRE [ tptr t_lock ]
        PROP ()
        PARAMS (ptr_of h)
-       SEP (weak_exclusive_mpred R && emp; lock_inv sh h R; P; lock_inv sh h R * P -* Q * R)
+       SEP (<affine> (R ∗ R -∗ False); lock_inv sh h R; P; lock_inv sh h R * P -* Q * R)
     POST [ tvoid ]
        PROP ()
        LOCAL ()
-       SEP (|> Q).
+       SEP (▷ Q).
   Next Obligation.
   Proof.
     repeat intro.
     destruct x as ((((?, ?), ?), ?), ?); simpl.
     unfold PROPx, PARAMSx, GLOBALSx, LOCALx, SEPx, argsassert2assert; simpl; rewrite !approx_andp; do 3 f_equal;
-      rewrite -> !sepcon_emp, ?approx_sepcon, ?approx_idem.
+      rewrite -> !bi.sep_emp, ?approx_sepcon, ?approx_idem.
     f_equal.
     { rewrite !approx_andp; f_equal.
       apply exclusive_mpred_super_non_expansive. }
@@ -769,7 +564,7 @@ Obligation Tactic := try solve_proper.*)
     repeat intro.
     destruct x as ((((?, ?), ?), ?), ?); simpl.
     unfold PROPx, LOCALx, SEPx; simpl; rewrite !approx_andp; do 2 f_equal;
-      rewrite -> !sepcon_emp, ?approx_sepcon, ?approx_idem.
+      rewrite -> !bi.sep_emp, ?approx_sepcon, ?approx_idem.
     setoid_rewrite later_nonexpansive; rewrite approx_idem; auto.
   Qed.
 
@@ -778,8 +573,8 @@ Obligation Tactic := try solve_proper.*)
     apply prove_funspec_sub.
     split; auto. intros. simpl in *. destruct x2 as ((((sh, h), R), P), Q). Intros.
     unfold rev_curry, tcurry. iIntros "H !>". iExists nil.
-    iExists (@ptr_of atomic_impl h, |> Q), emp. simpl in *.
-    rewrite emp_sepcon. iSplit.
+    iExists (@ptr_of atomic_impl h, ▷ Q), emp. simpl in *.
+    rewrite bi.emp_sep. iSplit.
     - unfold PROPx, PARAMSx, GLOBALSx, LOCALx, SEPx, argsassert2assert; simpl.
       iDestruct "H" as "(_ & % & _ & H)".
       do 4 (iSplit; auto).
@@ -802,7 +597,7 @@ Obligation Tactic := try solve_proper.*)
           iMod "Hclose'"; iMod ("Hclose" with "[-]"); last done.
           iLeft; unfold inv_for_lock; iExists false; iFrame; auto.
       + iPoseProof ("H4" with "[$H2 $H3]") as "[$ HR]"; auto.
-        iAssert (|>FF) with "[H5 R HR]" as ">[]".
+        iAssert (▷FF) with "[H5 R HR]" as ">[]".
         iNext; iApply weak_exclusive_conflict; iFrame; iFrame.
       + iDestruct (own_valid_2 with "[$H2 $inv]") as %(? & J & ?).
         apply sepalg.join_comm, join_Tsh in J as []; contradiction.
@@ -816,7 +611,7 @@ Obligation Tactic := try solve_proper.*)
     split; auto. intros. simpl in *. destruct x2 as ((sh, h), R). Intros.
     unfold rev_curry, tcurry. iIntros "H !>". iExists nil.
     iExists (@ptr_of atomic_impl h, @lock_inv atomic_impl sh h R), emp. simpl in *.
-    rewrite emp_sepcon. iSplit.
+    rewrite bi.emp_sep. iSplit.
     - unfold PROPx, PARAMSx, GLOBALSx, LOCALx, SEPx, argsassert2assert; simpl.
       iDestruct "H" as "([% _] & % & _ & H)".
       do 4 (iSplit; auto).
@@ -838,7 +633,7 @@ Obligation Tactic := try solve_proper.*)
         * iIntros (_) "[H1 _]". iDestruct "H5" as "_". iDestruct "R" as ">_". iFrame "H H2".
           iMod "Hclose'"; iApply "Hclose".
           iLeft; unfold inv_for_lock; iExists false; iFrame; auto.
-      + iAssert (|>FF) with "[H5 R H3]" as ">[]".
+      + iAssert (▷FF) with "[H5 R H3]" as ">[]".
         iNext; iApply weak_exclusive_conflict; iFrame; iFrame.
       + iDestruct (own_valid_2 with "[$H2 $inv]") as %(? & J & ?).
         apply sepalg.join_comm, join_Tsh in J as []; contradiction.
@@ -862,7 +657,7 @@ Obligation Tactic := try solve_proper.*)
     repeat intro.
     destruct x as ((?, ?), ?); simpl.
     unfold PROPx, PARAMSx, GLOBALSx, LOCALx, SEPx, argsassert2assert; simpl; rewrite !approx_andp; do 3 f_equal;
-      rewrite -> !sepcon_emp, ?approx_sepcon, ?approx_idem.
+      rewrite -> !bi.sep_emp, ?approx_sepcon, ?approx_idem.
     f_equal.
     setoid_rewrite (@lock_inv_super_non_expansive atomic_impl); do 2 f_equal.
     rewrite !approx_sepcon approx_idem; auto.
@@ -874,8 +669,6 @@ Obligation Tactic := try solve_proper.*)
     reflexivity.
   Qed.
 
-  #[local] Hint Resolve self_part_exclusive : core.
-
   Lemma release_self : funspec_sub (snd release_spec) release_spec_self.
   Proof.
     apply prove_funspec_sub.
@@ -883,7 +676,7 @@ Obligation Tactic := try solve_proper.*)
     unfold rev_curry, tcurry. iIntros "H !>". iExists nil.
     destruct h as ((v, N), g).
     iExists (v, emp), emp. simpl in *.
-    rewrite emp_sepcon. iSplit.
+    rewrite bi.emp_sep. iSplit.
     - unfold PROPx, PARAMSx, GLOBALSx, LOCALx, SEPx, argsassert2assert; simpl.
       iDestruct "H" as "(_ & % & _ & H)".
       do 4 (iSplit; auto).
@@ -919,7 +712,7 @@ Obligation Tactic := try solve_proper.*)
     split; auto. intros. simpl in *. destruct x2 as ((h, R), P). Intros.
     iIntros "H". iExists nil, (@ptr_of atomic_impl h), P.
     unfold PROPx, PARAMSx, GLOBALSx, LOCALx, SEPx, argsassert2assert; simpl.
-    rewrite !sepcon_emp. iDestruct "H" as "(_ & % & % & H1 & HP & R)".
+    rewrite !bi.sep_emp. iDestruct "H" as "(_ & % & % & H1 & HP & R)".
     unfold lock_inv; simpl; unfold atomic_lock_inv; destruct h as ((v, i), g).
     iDestruct "H1" as "(([% %] & #H) & H2)".
     iInv "H" as "[inv | inv]" "Hclose".
@@ -933,9 +726,9 @@ Obligation Tactic := try solve_proper.*)
       iExists _; iApply "a".
     - iPureIntro; intros; Intros; cancel.
       apply andp_left2; auto.
-    - iAssert (|>FF) with "[R HP HR H2]" as ">[]".
+    - iAssert (▷FF) with "[R HP HR H2]" as ">[]".
       iNext; iApply "R"; iFrame; iSplit; auto.
-    - iAssert (|>FF) with "[H2 inv]" as ">[]".
+    - iAssert (▷FF) with "[H2 inv]" as ">[]".
       iNext; iApply cinv_own_excl; [|iFrame]; auto.
   Qed.
 
@@ -960,7 +753,7 @@ Obligation Tactic := try solve_proper.*)
     repeat intro.
     destruct x as (((?, ?), ?), ?); simpl.
     unfold PROPx, PARAMSx, GLOBALSx, LOCALx, SEPx, argsassert2assert; simpl; rewrite !approx_andp; do 3 f_equal;
-      rewrite -> !sepcon_emp, ?approx_sepcon, ?approx_idem.
+      rewrite -> !bi.sep_emp, ?approx_sepcon, ?approx_idem.
     f_equal.
     setoid_rewrite (@lock_inv_super_non_expansive atomic_impl); do 2 f_equal.
     rewrite !approx_sepcon approx_idem; auto.
@@ -970,12 +763,7 @@ Obligation Tactic := try solve_proper.*)
     repeat intro.
     destruct x as (((?, ?), ?), ?); simpl.
     unfold PROPx, LOCALx, SEPx; simpl; rewrite !approx_andp; do 2 f_equal;
-      rewrite -> !sepcon_emp, ?approx_sepcon, ?approx_idem.
-  Qed.
-
-  Lemma lock_inv_share : forall sh h R, lock_inv sh h R |-- !!(sh <> Share.bot /\ isptr (ptr_of h)).
-  Proof.
-    intros; destruct h as ((?, ?), ?); unfold lock_inv; simpl; Intros; entailer!.
+      rewrite -> !bi.sep_emp, ?approx_sepcon, ?approx_idem.
   Qed.
 
   Lemma freelock_self : funspec_sub (snd freelock_spec) freelock_spec_self.
@@ -986,7 +774,7 @@ Obligation Tactic := try solve_proper.*)
     iIntros "H !>".
     iExists nil, (h, self_part sh2 h * R, emp), emp.
     unfold PROPx, PARAMSx, GLOBALSx, LOCALx, SEPx, argsassert2assert; simpl.
-    rewrite !emp_sepcon !sepcon_emp.
+    rewrite !bi.emp_sep !bi.sep_emp.
     iDestruct "H" as "((% & % & _) & % & % & H)".
     iSplit; [do 3 (iSplit; [auto|])|].
     - iAssert (⌜sh1 <> Share.bot⌝) with "[H]" as %?.
@@ -998,18 +786,10 @@ Obligation Tactic := try solve_proper.*)
       iDestruct "H" as "[[[_ g1] [_ g2]] _]".
       iApply (cinv_own_excl with "[$g1 $g2]"); auto.
     - iPureIntro; intros; Intros.
-      rewrite emp_sepcon; apply andp_left2; auto.
+      rewrite bi.emp_sep; apply andp_left2; auto.
   Qed.
 
 End PROOFS.
-
-Notation selflock R sh h := (self_part sh h * R).
-
-#[export] Hint Resolve self_part_exclusive : core.
-#[export] Hint Resolve lock_inv_share : saturate_local.
-
-Ltac lock_props ::= match goal with |-context[weak_exclusive_mpred ?P && _] => sep_apply (exclusive_weak_exclusive P); [auto with share | try timeout 20 cancel]
-  | |-context[weak_exclusive_mpred' ?P && _] => sep_apply (exclusive_weak_exclusive' P); [auto with share | try timeout 20 cancel] end.
 
 (* when interacting with atomic updates, we need to unfold the definition of lock_inv and split its pieces *)
 Ltac unfold_lock_inv := match goal with |-context[lock_inv _ ?h _] =>
