atomics/general_atomics.v
@@ -14,7 +14,7 @@ Definition tele_unwrap {A} (x : tele_arg (TeleS (fun _ : A => TeleO))) :=
   | TeleArgCons x _ => x
   end.
 
-Context `{!VSTGS OK_ty Σ}.
+Context `{!heapGS Σ}.
 
 Definition atomic_shift {A B} (a : A -d> mpred) Eo Ei (b : A -d> B -d> mpred) (Q : B -d> mpred) : mpred :=
   atomic_update(TA := [tele _ : A]) (TB := [tele _ : B]) Eo Ei (λ.. x, a (tele_unwrap x)) (λ.. x y, b (tele_unwrap x) (tele_unwrap y)) (λ.. x y, Q (tele_unwrap y)).
@@ -173,10 +173,10 @@ Global Hint Resolve empty_subseteq : core.
 Definition atomic_spec_type W T := ProdType W (ArrowType (ConstType T) Mpred).
 Definition atomic_spec_type0 W := ProdType W Mpred.
 
-Program Definition atomic_spec_pre' `{!VSTGS OK_ty Σ} {A T} W
+Program Definition atomic_spec_pre' `{!heapGS Σ} {A T} W
   (P : dtfr W -n> _) (L : dtfr W -n> _) (G : dtfr W -n> leibnizO (list globals)) (R : dtfr W -n> _) (S2 : dtfr W -n> _)
   (E : dtfr W -n> leibnizO coPset) (SQ : dtfr W -n> _) :
-  (prodO (@dtfr Σ W) (T -d> mpred)) -n> argsEnviron -d> mpred :=
+  (prodO (@dtfr Σ W) (T -d> iProp Σ)) -n> argsEnviron -d> mpred :=
   λne '(w, Q),
     PROPx (P w) (PARAMSx (L w) (GLOBALSx (G w)
      (SEPx (atomic_shift(A := A) (S2 w) (⊤ ∖ E w) ∅ (SQ w) Q :: R w)))).
@@ -191,7 +191,7 @@ Proof.
   rewrite Hw H //.
 Qed.
 
-Program Definition atomic_spec_pre0 `{!VSTGS OK_ty Σ} {A} W
+Program Definition atomic_spec_pre0 `{!heapGS Σ} {A} W
   (P : dtfr W -n> _) (L : dtfr W -n> _) (G : dtfr W -n> leibnizO (list globals)) (R : dtfr W -n> _) (S2 : dtfr W -n> _)
   (E : dtfr W -n> leibnizO coPset) (SQ : dtfr W -n> _) :
   (prodO (@dtfr Σ W) mpred) -n> argsEnviron -d> mpred :=
@@ -209,7 +209,7 @@ Proof.
   rewrite Hw; repeat f_equiv; solve_proper.
 Qed.
 
-Program Definition atomic_spec_post' `{!VSTGS OK_ty Σ} {T} W
+Program Definition atomic_spec_post' `{!heapGS Σ} {T} W
   (L : dtfr W -n> _ -d> leibnizO _) (R : dtfr W -n> _ -d> _) :
   (prodO (@dtfr Σ W) (T -d> mpred)) -n> environ -d> mpred :=
     λne '(w, Q),
@@ -224,7 +224,7 @@ Proof.
   unshelve rewrite -> (ofe_mor_ne _ _ R n); done.
 Qed.
 
-Program Definition atomic_spec_post0 `{!VSTGS OK_ty Σ} W
+Program Definition atomic_spec_post0 `{!heapGS Σ} W
   (L : dtfr W -n> leibnizO _) (R : dtfr W -n> _) :
   (prodO (@dtfr Σ W) mpred) -n> environ -d> mpred :=
     λne '(w, Q),
@@ -240,7 +240,7 @@ Qed.
 
 (* A is the type of the abstract data. T is the type quantified over in the postcondition.
    W is the TypeTree of the witness for the rest of the function. *)
-Program Definition atomic_spec `{!VSTGS OK_ty Σ} {A T} {t : Inhabitant T} W args (tz : type)
+Program Definition atomic_spec `{!heapGS Σ} {A T} {t : Inhabitant T} W args (tz : type)
   (la : dtfr W -n> list.listO (leibnizO val)) (P : dtfr W -n> mpred) (G : dtfr W -n> leibnizO (list globals))
   (Qp : T -> dtfr W -n> mpred) (a : dtfr W -n> _) (lb : dtfr W -n> T -d> leibnizO (list localdef))
         (b : dtfr W -n> _) (E : dtfr W -n> leibnizO coPset)
@@ -322,468 +322,470 @@ Definition rev_curry {A B} (f : tuple_type A -> B) : tuple_type_rev A -> B
 Notation "'ATOMIC' 'TYPE' W 'OBJ' x : A 'INVS' E 'WITH' x1 , .. , xn 'PRE'  [ u , .. , v ] 'PROP' ( Px ; .. ; Py ) 'PARAMS' ( Lx ; .. ; Ly ) 'GLOBALS' ( Gx ; .. ; Gy ) 'SEP' ( S1x ; .. ; S1y ) '|' S2 'POST' [ tz ] 'EX' r : T , 'PROP' () 'LOCAL' ( LQx ; .. ; LQy ) 'SEP' ( SPx ; .. ; SPy ) '|' ( SQx ; .. ; SQy )" :=
   (mk_funspec (pair (cons u%type .. (cons v%type nil) ..) tz) cc_default ⊤ (atomic_spec_type W T)
    (atomic_spec_pre'(A := A)(T := T) W
-      (OfeMor (rev_curry (tcurry (fun x1 => .. (tcurry (fun xn (_ : tuple_type tnil) => (cons Px%type .. (cons Py%type nil) ..))) ..))))
-      (OfeMor (rev_curry (tcurry (fun x1 => .. (tcurry (fun xn (_ : tuple_type tnil) => (cons Lx%type .. (cons Ly%type nil) ..))) ..))))
-      (OfeMor (rev_curry (tcurry (fun x1 => .. (tcurry (fun xn (_ : tuple_type tnil) => (cons Gx .. (cons Gy nil) ..))) ..))))
-      (OfeMor (rev_curry (tcurry (fun x1 => .. (tcurry (fun xn (_ : tuple_type tnil) => (cons S1x%I .. (cons S1y%I nil) ..))) ..))))
-      (OfeMor (rev_curry (tcurry (fun x1 => .. (tcurry (fun xn (_ : tuple_type tnil) x => S2)) ..))))
-      (OfeMor (rev_curry (tcurry (fun x1 => .. (tcurry (fun xn (_ : tuple_type tnil) => E)) ..))))
-      (OfeMor (rev_curry (tcurry (fun x1 => .. (tcurry (fun xn (_ : tuple_type tnil) x r => fold_right_sepcon (cons SQx%I .. (cons SQy%I nil) ..))) ..)))))
+      (OfeMor(ofe_mor_ne := _) (rev_curry (tcurry (fun x1 => .. (tcurry (fun xn (_ : tuple_type tnil) => (cons Px%type .. (cons Py%type nil) ..))) ..))))
+      (OfeMor(ofe_mor_ne := _) (rev_curry (tcurry (fun x1 => .. (tcurry (fun xn (_ : tuple_type tnil) => (cons Lx%type .. (cons Ly%type nil) ..))) ..))))
+      (OfeMor(ofe_mor_ne := _) (rev_curry (tcurry (fun x1 => .. (tcurry (fun xn (_ : tuple_type tnil) => (cons Gx .. (cons Gy nil) ..))) ..))))
+      (OfeMor(ofe_mor_ne := _) (rev_curry (tcurry (fun x1 => .. (tcurry (fun xn (_ : tuple_type tnil) => (cons S1x%I .. (cons S1y%I nil) ..))) ..))))
+      (OfeMor(ofe_mor_ne := _) (rev_curry (tcurry (fun x1 => .. (tcurry (fun xn (_ : tuple_type tnil) x => S2)) ..))))
+      (OfeMor(ofe_mor_ne := _) (rev_curry (tcurry (fun x1 => .. (tcurry (fun xn (_ : tuple_type tnil) => E)) ..))))
+      (OfeMor(ofe_mor_ne := _) (rev_curry (tcurry (fun x1 => .. (tcurry (fun xn (_ : tuple_type tnil) x r => fold_right_sepcon (cons SQx%I .. (cons SQy%I nil) ..))) ..)))))
    (atomic_spec_post'(T := T) W
-      (OfeMor (rev_curry (tcurry (fun x1 => .. (tcurry (fun xn (_ : tuple_type tnil) r => (cons LQx%assert3 .. (cons LQy%assert3 nil) ..))) ..))))
-      (OfeMor (rev_curry (tcurry (fun x1 => .. (tcurry (fun xn (_ : tuple_type tnil) r => (cons SPx%assert3 .. (cons SPy%assert3 nil) ..))) ..))))))
+      (OfeMor(ofe_mor_ne := _) (rev_curry (tcurry (fun x1 => .. (tcurry (fun xn (_ : tuple_type tnil) r => (cons LQx%assert3 .. (cons LQy%assert3 nil) ..))) ..))))
+      (OfeMor(ofe_mor_ne := _) (rev_curry (tcurry (fun x1 => .. (tcurry (fun xn (_ : tuple_type tnil) r => (cons SPx%assert3 .. (cons SPy%assert3 nil) ..))) ..))))))
   (at level 200, x1 closed binder, xn closed binder, x at level 0, E at level 0, S2 at level 0, r at level 0, T at level 0).
 
 Notation "'ATOMIC' 'TYPE' W 'OBJ' x 'INVS' E 'WITH' x1 , .. , xn 'PRE'  [ u , .. , v ] 'PROP' ( Px ; .. ; Py ) 'PARAMS' ( Lx ; .. ; Ly ) 'GLOBALS' ( Gx ; .. ; Gy ) 'SEP' ( S1x ; .. ; S1y ) '|' S2 'POST' [ tz ] 'EX' r : T , 'PROP' () 'LOCAL' ( LQx ; .. ; LQy ) 'SEP' ( SPx ; .. ; SPy ) '|' ( SQx ; .. ; SQy )" :=
   (mk_funspec (pair (cons u%type .. (cons v%type nil) ..) tz) cc_default ⊤ (atomic_spec_type W T)
    (atomic_spec_pre'(T := T) W
-      (OfeMor (rev_curry (tcurry (fun x1 => .. (tcurry (fun xn (_ : tuple_type tnil) => (cons Px%type .. (cons Py%type nil) ..))) ..))))
-      (OfeMor (rev_curry (tcurry (fun x1 => .. (tcurry (fun xn (_ : tuple_type tnil) => (cons Lx%type .. (cons Ly%type nil) ..))) ..))))
-      (OfeMor (rev_curry (tcurry (fun x1 => .. (tcurry (fun xn (_ : tuple_type tnil) => (cons Gx .. (cons Gy nil) ..))) ..))))
-      (OfeMor (rev_curry (tcurry (fun x1 => .. (tcurry (fun xn (_ : tuple_type tnil) => (cons S1x%I .. (cons S1y%I nil) ..))) ..))))
-      (OfeMor (rev_curry (tcurry (fun x1 => .. (tcurry (fun xn (_ : tuple_type tnil) x => S2)) ..))))
-      (OfeMor (rev_curry (tcurry (fun x1 => .. (tcurry (fun xn (_ : tuple_type tnil) => E)) ..))))
-      (OfeMor (rev_curry (tcurry (fun x1 => .. (tcurry (fun xn (_ : tuple_type tnil) x r => fold_right_sepcon (cons SQx%I .. (cons SQy%I nil) ..))) ..)))))
+      (OfeMor(ofe_mor_ne := _) (rev_curry (tcurry (fun x1 => .. (tcurry (fun xn (_ : tuple_type tnil) => (cons Px%type .. (cons Py%type nil) ..))) ..))))
+      (OfeMor(ofe_mor_ne := _) (rev_curry (tcurry (fun x1 => .. (tcurry (fun xn (_ : tuple_type tnil) => (cons Lx%type .. (cons Ly%type nil) ..))) ..))))
+      (OfeMor(ofe_mor_ne := _) (rev_curry (tcurry (fun x1 => .. (tcurry (fun xn (_ : tuple_type tnil) => (cons Gx .. (cons Gy nil) ..))) ..))))
+      (OfeMor(ofe_mor_ne := _) (rev_curry (tcurry (fun x1 => .. (tcurry (fun xn (_ : tuple_type tnil) => (cons S1x%I .. (cons S1y%I nil) ..))) ..))))
+      (OfeMor(ofe_mor_ne := _) (rev_curry (tcurry (fun x1 => .. (tcurry (fun xn (_ : tuple_type tnil) x => S2)) ..))))
+      (OfeMor(ofe_mor_ne := _) (rev_curry (tcurry (fun x1 => .. (tcurry (fun xn (_ : tuple_type tnil) => E)) ..))))
+      (OfeMor(ofe_mor_ne := _) (rev_curry (tcurry (fun x1 => .. (tcurry (fun xn (_ : tuple_type tnil) x r => fold_right_sepcon (cons SQx%I .. (cons SQy%I nil) ..))) ..)))))
    (atomic_spec_post' W
-      (OfeMor (rev_curry (tcurry (fun x1 => .. (tcurry (fun xn (_ : tuple_type tnil) r => (cons LQx%assert3 .. (cons LQy%assert3 nil) ..))) ..))))
-      (OfeMor (rev_curry (tcurry (fun x1 => .. (tcurry (fun xn (_ : tuple_type tnil) r => (cons SPx%assert3 .. (cons SPy%assert3 nil) ..))) ..))))))
+      (OfeMor(ofe_mor_ne := _) (rev_curry (tcurry (fun x1 => .. (tcurry (fun xn (_ : tuple_type tnil) r => (cons LQx%assert3 .. (cons LQy%assert3 nil) ..))) ..))))
+      (OfeMor(ofe_mor_ne := _) (rev_curry (tcurry (fun x1 => .. (tcurry (fun xn (_ : tuple_type tnil) r => (cons SPx%assert3 .. (cons SPy%assert3 nil) ..))) ..))))))
   (at level 200, x1 closed binder, xn closed binder, x at level 0, E at level 0, S2 at level 0, r at level 0, T at level 0).
 
 Notation "'ATOMIC' 'TYPE' W 'OBJ' x 'INVS' E 'WITH' x1 , .. , xn 'PRE'  [ u , .. , v ] 'PROP' ( Px ; .. ; Py ) 'PARAMS' ( Lx ; .. ; Ly ) 'GLOBALS' ( Gx ; .. ; Gy ) 'SEP' ( S1x ; .. ; S1y ) '|' S2 'POST' [ tz ] 'EX' r : T , 'PROP' () 'LOCAL' () 'SEP' ( SPx ; .. ; SPy ) '|' ( SQx ; .. ; SQy )" :=
   (mk_funspec (pair (cons u%type .. (cons v%type nil) ..) tz) cc_default ⊤ (atomic_spec_type W T)
    (atomic_spec_pre'(T := T) W
-      (OfeMor (rev_curry (tcurry (fun x1 => .. (tcurry (fun xn (_ : tuple_type tnil) => (cons Px%type .. (cons Py%type nil) ..))) ..))))
-      (OfeMor (rev_curry (tcurry (fun x1 => .. (tcurry (fun xn (_ : tuple_type tnil) => (cons Lx%type .. (cons Ly%type nil) ..))) ..))))
-      (OfeMor (rev_curry (tcurry (fun x1 => .. (tcurry (fun xn (_ : tuple_type tnil) => (cons Gx .. (cons Gy nil) ..))) ..))))
-      (OfeMor (rev_curry (tcurry (fun x1 => .. (tcurry (fun xn (_ : tuple_type tnil) => (cons S1x%I .. (cons S1y%I nil) ..))) ..))))
-      (OfeMor (rev_curry (tcurry (fun x1 => .. (tcurry (fun xn (_ : tuple_type tnil) x => S2)) ..))))       (OfeMor (rev_curry (tcurry (fun x1 => .. (tcurry (fun xn (_ : tuple_type tnil) => E)) ..))))
-      (OfeMor (rev_curry (tcurry (fun x1 => .. (tcurry (fun xn (_ : tuple_type tnil) x r => fold_right_sepcon (cons SQx%I .. (cons SQy%I nil) ..))) ..)))))
+      (OfeMor(ofe_mor_ne := _) (rev_curry (tcurry (fun x1 => .. (tcurry (fun xn (_ : tuple_type tnil) => (cons Px%type .. (cons Py%type nil) ..))) ..))))
+      (OfeMor(ofe_mor_ne := _) (rev_curry (tcurry (fun x1 => .. (tcurry (fun xn (_ : tuple_type tnil) => (cons Lx%type .. (cons Ly%type nil) ..))) ..))))
+      (OfeMor(ofe_mor_ne := _) (rev_curry (tcurry (fun x1 => .. (tcurry (fun xn (_ : tuple_type tnil) => (cons Gx .. (cons Gy nil) ..))) ..))))
+      (OfeMor(ofe_mor_ne := _) (rev_curry (tcurry (fun x1 => .. (tcurry (fun xn (_ : tuple_type tnil) => (cons S1x%I .. (cons S1y%I nil) ..))) ..))))
+      (OfeMor(ofe_mor_ne := _) (rev_curry (tcurry (fun x1 => .. (tcurry (fun xn (_ : tuple_type tnil) x => S2)) ..))))       (OfeMor(ofe_mor_ne := _) (rev_curry (tcurry (fun x1 => .. (tcurry (fun xn (_ : tuple_type tnil) => E)) ..))))
+      (OfeMor(ofe_mor_ne := _) (rev_curry (tcurry (fun x1 => .. (tcurry (fun xn (_ : tuple_type tnil) x r => fold_right_sepcon (cons SQx%I .. (cons SQy%I nil) ..))) ..)))))
    (atomic_spec_post' W
-      (OfeMor (rev_curry (tcurry (fun x1 => .. (tcurry (fun xn (_ : tuple_type tnil) r => nil)) ..))))
-      (OfeMor (rev_curry (tcurry (fun x1 => .. (tcurry (fun xn (_ : tuple_type tnil) r => (cons SPx%assert5%assert3 .. (cons SPy%assert5%assert3 nil) ..))) ..))))))
+      (OfeMor(ofe_mor_ne := _)(B := leibnizO (list localdef)) (rev_curry (tcurry (fun x1 => .. (tcurry (fun xn (_ : tuple_type tnil) r => nil)) ..))))
+      (OfeMor(ofe_mor_ne := _) (rev_curry (tcurry (fun x1 => .. (tcurry (fun xn (_ : tuple_type tnil) r => (cons SPx%assert5%assert3 .. (cons SPy%assert5%assert3 nil) ..))) ..))))))
   (at level 200, x1 closed binder, xn closed binder, x at level 0, E at level 0, S2 at level 0, r at level 0, T at level 0).
 
 Notation "'ATOMIC' 'TYPE' W 'OBJ' x 'INVS' E 'WITH' x1 , .. , xn 'PRE'  [ u , .. , v ] 'PROP' ( Px ; .. ; Py ) 'PARAMS' ( Lx ; .. ; Ly ) 'GLOBALS' ( Gx ; .. ; Gy ) 'SEP' ( S1x ; .. ; S1y ) '|' S2 'POST' [ tz ] 'PROP' () 'LOCAL' ( LQx ; .. ; LQy ) 'SEP' ( SPx ; .. ; SPy ) '|' ( SQx ; .. ; SQy )" :=
   (mk_funspec (pair (cons u%type .. (cons v%type nil) ..) tz) cc_default ⊤ (atomic_spec_type0 W)
    (atomic_spec_pre0 W
-      (OfeMor (rev_curry (tcurry (fun x1 => .. (tcurry (fun xn (_ : tuple_type tnil) => (cons Px%type .. (cons Py%type nil) ..))) ..))))
-      (OfeMor (rev_curry (tcurry (fun x1 => .. (tcurry (fun xn (_ : tuple_type tnil) => (cons Lx%type .. (cons Ly%type nil) ..))) ..))))
-      (OfeMor (rev_curry (tcurry (fun x1 => .. (tcurry (fun xn (_ : tuple_type tnil) => (cons Gx .. (cons Gy nil) ..))) ..))))
-      (OfeMor (rev_curry (tcurry (fun x1 => .. (tcurry (fun xn (_ : tuple_type tnil) => (cons S1x%I .. (cons S1y%I nil) ..))) ..))))
-      (OfeMor (rev_curry (tcurry (fun x1 => .. (tcurry (fun xn (_ : tuple_type tnil) x => S2)) ..))))
-      (OfeMor (rev_curry (tcurry (fun x1 => .. (tcurry (fun xn (_ : tuple_type tnil) => E)) ..))))
-      (OfeMor (rev_curry (tcurry (fun x1 => .. (tcurry (fun xn (_ : tuple_type tnil) x _ => fold_right_sepcon (cons SQx%I .. (cons SQy%I nil) ..))) ..)))))
+      (OfeMor(ofe_mor_ne := _) (rev_curry (tcurry (fun x1 => .. (tcurry (fun xn (_ : tuple_type tnil) => (cons Px%type .. (cons Py%type nil) ..))) ..))))
+      (OfeMor(ofe_mor_ne := _) (rev_curry (tcurry (fun x1 => .. (tcurry (fun xn (_ : tuple_type tnil) => (cons Lx%type .. (cons Ly%type nil) ..))) ..))))
+      (OfeMor(ofe_mor_ne := _) (rev_curry (tcurry (fun x1 => .. (tcurry (fun xn (_ : tuple_type tnil) => (cons Gx .. (cons Gy nil) ..))) ..))))
+      (OfeMor(ofe_mor_ne := _) (rev_curry (tcurry (fun x1 => .. (tcurry (fun xn (_ : tuple_type tnil) => (cons S1x%I .. (cons S1y%I nil) ..))) ..))))
+      (OfeMor(ofe_mor_ne := _) (rev_curry (tcurry (fun x1 => .. (tcurry (fun xn (_ : tuple_type tnil) x => S2)) ..))))
+      (OfeMor(ofe_mor_ne := _) (rev_curry (tcurry (fun x1 => .. (tcurry (fun xn (_ : tuple_type tnil) => E)) ..))))
+      (OfeMor(ofe_mor_ne := _) (rev_curry (tcurry (fun x1 => .. (tcurry (fun xn (_ : tuple_type tnil) x _ => fold_right_sepcon (cons SQx%I .. (cons SQy%I nil) ..))) ..)))))
   (atomic_spec_post0 W
-      (OfeMor (rev_curry (tcurry (fun x1 => .. (tcurry (fun xn (_ : tuple_type tnil) => (cons LQx%assert3 .. (cons LQy%assert3 nil) ..))) ..))))
-      (OfeMor (rev_curry (tcurry (fun x1 => .. (tcurry (fun xn (_ : tuple_type tnil) => (cons SPx%assert3 .. (cons SPy%assert3 nil) ..))) ..))))))
+      (OfeMor(ofe_mor_ne := _) (rev_curry (tcurry (fun x1 => .. (tcurry (fun xn (_ : tuple_type tnil) => (cons LQx%assert3 .. (cons LQy%assert3 nil) ..))) ..))))
+      (OfeMor(ofe_mor_ne := _) (rev_curry (tcurry (fun x1 => .. (tcurry (fun xn (_ : tuple_type tnil) => (cons SPx%assert3 .. (cons SPy%assert3 nil) ..))) ..))))))
   (at level 200, x1 closed binder, xn closed binder, x at level 0, E at level 0, S2 at level 0).
 
 Notation "'ATOMIC' 'TYPE' W 'OBJ' x 'INVS' E 'WITH' x1 , .. , xn 'PRE'  [ u , .. , v ] 'PROP' ( Px ; .. ; Py ) 'PARAMS' ( Lx ; .. ; Ly ) 'GLOBALS' ( Gx ; .. ; Gy ) 'SEP' ( S1x ; .. ; S1y ) '|' S2 'POST' [ tz ] 'PROP' () 'LOCAL' () 'SEP' ( SPx ; .. ; SPy ) '|' ( SQx ; .. ; SQy )" :=
   (mk_funspec (pair (cons u%type .. (cons v%type nil) ..) tz) cc_default ⊤ (atomic_spec_type0 W)
    (atomic_spec_pre0 W
-      (OfeMor (rev_curry (tcurry (fun x1 => .. (tcurry (fun xn (_ : tuple_type tnil) => (cons Px%type .. (cons Py%type nil) ..))) ..))))
-      (OfeMor (rev_curry (tcurry (fun x1 => .. (tcurry (fun xn (_ : tuple_type tnil) => (cons Lx%type .. (cons Ly%type nil) ..))) ..))))
-      (OfeMor (rev_curry (tcurry (fun x1 => .. (tcurry (fun xn (_ : tuple_type tnil) => (cons Gx .. (cons Gy nil) ..))) ..))))
-      (OfeMor (rev_curry (tcurry (fun x1 => .. (tcurry (fun xn (_ : tuple_type tnil) => (cons S1x%I .. (cons S1y%I nil) ..))) ..))))
-      (OfeMor (rev_curry (tcurry (fun x1 => .. (tcurry (fun xn (_ : tuple_type tnil) x => S2)) ..))))
-      (OfeMor (rev_curry (tcurry (fun x1 => .. (tcurry (fun xn (_ : tuple_type tnil) => E)) ..))))
-      (OfeMor (rev_curry (tcurry (fun x1 => .. (tcurry (fun xn (_ : tuple_type tnil) x _ => fold_right_sepcon (cons SQx%I .. (cons SQy%I nil) ..))) ..)))))
+      (OfeMor(ofe_mor_ne := _) (rev_curry (tcurry (fun x1 => .. (tcurry (fun xn (_ : tuple_type tnil) => (cons Px%type .. (cons Py%type nil) ..))) ..))))
+      (OfeMor(ofe_mor_ne := _) (rev_curry (tcurry (fun x1 => .. (tcurry (fun xn (_ : tuple_type tnil) => (cons Lx%type .. (cons Ly%type nil) ..))) ..))))
+      (OfeMor(ofe_mor_ne := _) (rev_curry (tcurry (fun x1 => .. (tcurry (fun xn (_ : tuple_type tnil) => (cons Gx .. (cons Gy nil) ..))) ..))))
+      (OfeMor(ofe_mor_ne := _) (rev_curry (tcurry (fun x1 => .. (tcurry (fun xn (_ : tuple_type tnil) => (cons S1x%I .. (cons S1y%I nil) ..))) ..))))
+      (OfeMor(ofe_mor_ne := _) (rev_curry (tcurry (fun x1 => .. (tcurry (fun xn (_ : tuple_type tnil) x => S2)) ..))))
+      (OfeMor(ofe_mor_ne := _) (rev_curry (tcurry (fun x1 => .. (tcurry (fun xn (_ : tuple_type tnil) => E)) ..))))
+      (OfeMor(ofe_mor_ne := _) (rev_curry (tcurry (fun x1 => .. (tcurry (fun xn (_ : tuple_type tnil) x _ => fold_right_sepcon (cons SQx%I .. (cons SQy%I nil) ..))) ..)))))
   (atomic_spec_post0 W
-      (OfeMor (rev_curry (tcurry (fun x1 => .. (tcurry (fun xn (_ : tuple_type tnil) => nil)) ..))))
-      (OfeMor (rev_curry (tcurry (fun x1 => .. (tcurry (fun xn (_ : tuple_type tnil) => (cons SPx%assert5%assert3 .. (cons SPy%assert5%assert3 nil) ..))) ..))))))
+      (OfeMor(ofe_mor_ne := _)(B := leibnizO (list localdef)) (rev_curry (tcurry (fun x1 => .. (tcurry (fun xn (_ : tuple_type tnil) => nil)) ..))))
+      (OfeMor(ofe_mor_ne := _) (rev_curry (tcurry (fun x1 => .. (tcurry (fun xn (_ : tuple_type tnil) => (cons SPx%assert5%assert3 .. (cons SPy%assert5%assert3 nil) ..))) ..))))))
   (at level 200, x1 closed binder, xn closed binder, x at level 0, E at level 0, S2 at level 0).
 
 Notation "'ATOMIC' 'TYPE' W 'INVS' E 'WITH' x1 , .. , xn 'PRE'  [ u , .. , v ] 'PROP' () 'PARAMS' ( Lx ; .. ; Ly ) 'SEP' () '|' S2 'POST' [ tz ] 'PROP' () 'LOCAL' () 'SEP' ( SPx ; .. ; SPy ) '|' ( SQx ; .. ; SQy )" :=
   (mk_funspec (pair (cons u%type .. (cons v%type nil) ..) tz) cc_default ⊤ (atomic_spec_type0 W)
    (atomic_spec_pre0 W
-      (OfeMor (rev_curry (tcurry (fun x1 => .. (tcurry (fun xn (_ : tuple_type tnil) => nil)) ..))))
-      (OfeMor (rev_curry (tcurry (fun x1 => .. (tcurry (fun xn (_ : tuple_type tnil) => (cons Lx%type .. (cons Ly%type nil) ..))) ..))))
-      (OfeMor (rev_curry (tcurry (fun x1 => .. (tcurry (fun xn (_ : tuple_type tnil) => nil)) ..))))
-      (OfeMor (rev_curry (tcurry (fun x1 => .. (tcurry (fun xn (_ : tuple_type tnil) => nil)) ..))))
-      (OfeMor (OfeMor (rev_curry (tcurry (fun x1 => .. (tcurry (fun xn (_ : tuple_type tnil) (_ : unit) => S2)) ..)))))
-      (OfeMor (rev_curry (tcurry (fun x1 => .. (tcurry (fun xn (_ : tuple_type tnil) => E)) ..))))
-      (OfeMor (rev_curry (tcurry (fun x1 => .. (tcurry (fun xn (_ : tuple_type tnil) (_ : unit) _ => fold_right_sepcon (cons SQx%I .. (cons SQy%I nil) ..))) ..)))))
+      (OfeMor(ofe_mor_ne := _) (rev_curry (tcurry (fun x1 => .. (tcurry (fun xn (_ : tuple_type tnil) => nil)) ..))))
+      (OfeMor(ofe_mor_ne := _) (rev_curry (tcurry (fun x1 => .. (tcurry (fun xn (_ : tuple_type tnil) => (cons Lx%type .. (cons Ly%type nil) ..))) ..))))
+      (OfeMor(B := leibnizO (list globals))(ofe_mor_ne := _) (rev_curry (tcurry (fun x1 => .. (tcurry (fun xn (_ : tuple_type tnil) => nil)) ..))))
+      (OfeMor(B := list mpred)(ofe_mor_ne := _) (rev_curry (tcurry (fun x1 => .. (tcurry (fun xn (_ : tuple_type tnil) => nil)) ..))))
+      (OfeMor(ofe_mor_ne := _) (rev_curry (tcurry (fun x1 => .. (tcurry (fun xn (_ : tuple_type tnil) (_ : unit) => S2)) ..))))
+      (OfeMor(ofe_mor_ne := _) (rev_curry (tcurry (fun x1 => .. (tcurry (fun xn (_ : tuple_type tnil) => E)) ..))))
+      (OfeMor(ofe_mor_ne := _) (rev_curry (tcurry (fun x1 => .. (tcurry (fun xn (_ : tuple_type tnil) (_ : unit) _ => fold_right_sepcon (cons SQx%I .. (cons SQy%I nil) ..))) ..)))))
   (atomic_spec_post0 W
-      (OfeMor (rev_curry (tcurry (fun x1 => .. (tcurry (fun xn (_ : tuple_type tnil) => nil)) ..))))
-      (OfeMor (rev_curry (tcurry (fun x1 => .. (tcurry (fun xn (_ : tuple_type tnil) => (cons SPx%assert5%assert3 .. (cons SPy%assert5%assert3 nil) ..))) ..))))))
+      (OfeMor(ofe_mor_ne := _) (rev_curry (tcurry (fun x1 => .. (tcurry (fun xn (_ : tuple_type tnil) => nil)) ..))))
+      (OfeMor(ofe_mor_ne := _) (rev_curry (tcurry (fun x1 => .. (tcurry (fun xn (_ : tuple_type tnil) => (cons SPx%assert5%assert3 .. (cons SPy%assert5%assert3 nil) ..))) ..))))))
   (at level 200, x1 closed binder, xn closed binder, E at level 0, S2 at level 0).
 
 Notation "'ATOMIC' 'TYPE' W 'INVS' E 'WITH' x1 , .. , xn 'PRE'  [ u , .. , v ] 'PROP' () 'PARAMS' ( Lx ; .. ; Ly ) 'SEP' ( S1x ; .. ; S1y ) '|' S2 'POST' [ tz ] 'PROP' () 'LOCAL' () 'SEP' () '|' ( SQx ; .. ; SQy )" :=
   (mk_funspec (pair (cons u%type .. (cons v%type nil) ..) tz) cc_default ⊤ (atomic_spec_type0 W)
    (atomic_spec_pre0 W
-      (OfeMor (rev_curry (tcurry (fun x1 => .. (tcurry (fun xn (_ : tuple_type tnil) => nil)) ..))))
-      (OfeMor (rev_curry (tcurry (fun x1 => .. (tcurry (fun xn (_ : tuple_type tnil) => (cons Lx%type .. (cons Ly%type nil) ..))) ..))))
-      (OfeMor (rev_curry (tcurry (fun x1 => .. (tcurry (fun xn (_ : tuple_type tnil) => nil)) ..))))
-      (OfeMor (rev_curry (tcurry (fun x1 => .. (tcurry (fun xn (_ : tuple_type tnil) => (cons S1x%I .. (cons S1y%I nil) ..))) ..))))
-      (OfeMor (OfeMor (rev_curry (tcurry (fun x1 => .. (tcurry (fun xn (_ : tuple_type tnil) (_ : unit) => S2)) ..))))       (OfeMor (rev_curry (tcurry (fun x1 => .. (tcurry (fun xn (_ : tuple_type tnil) => E)) ..)))))
-      (OfeMor (rev_curry (tcurry (fun x1 => .. (tcurry (fun xn (_ : tuple_type tnil) (_ : unit) _ => fold_right_sepcon (cons SQx%I .. (cons SQy%I nil) ..))) ..)))))
+      (OfeMor(ofe_mor_ne := _) (rev_curry (tcurry (fun x1 => .. (tcurry (fun xn (_ : tuple_type tnil) => nil)) ..))))
+      (OfeMor(ofe_mor_ne := _) (rev_curry (tcurry (fun x1 => .. (tcurry (fun xn (_ : tuple_type tnil) => (cons Lx%type .. (cons Ly%type nil) ..))) ..))))
+      (OfeMor(ofe_mor_ne := _)(B := leibnizO (list globals)) (rev_curry (tcurry (fun x1 => .. (tcurry (fun xn (_ : tuple_type tnil) => nil)) ..))))
+      (OfeMor(ofe_mor_ne := _) (rev_curry (tcurry (fun x1 => .. (tcurry (fun xn (_ : tuple_type tnil) => (cons S1x%I .. (cons S1y%I nil) ..))) ..))))
+      (OfeMor(ofe_mor_ne := _) (rev_curry (tcurry (fun x1 => .. (tcurry (fun xn (_ : tuple_type tnil) (_ : unit) => S2)) ..))))
+      (OfeMor(ofe_mor_ne := _) (rev_curry (tcurry (fun x1 => .. (tcurry (fun xn (_ : tuple_type tnil) => E)) ..))))
+      (OfeMor(ofe_mor_ne := _) (rev_curry (tcurry (fun x1 => .. (tcurry (fun xn (_ : tuple_type tnil) (_ : unit) _ => fold_right_sepcon (cons SQx%I .. (cons SQy%I nil) ..))) ..)))))
   (atomic_spec_post0 W
-      (OfeMor (rev_curry (tcurry (fun x1 => .. (tcurry (fun xn (_ : tuple_type tnil) => nil)) ..))))
-      (OfeMor (rev_curry (tcurry (fun x1 => .. (tcurry (fun xn (_ : tuple_type tnil) => nil)) ..))))))
+      (OfeMor(ofe_mor_ne := _)(B := leibnizO (list localdef)) (rev_curry (tcurry (fun x1 => .. (tcurry (fun xn (_ : tuple_type tnil) => nil)) ..))))
+      (OfeMor(ofe_mor_ne := _)(B := list mpred) (rev_curry (tcurry (fun x1 => .. (tcurry (fun xn (_ : tuple_type tnil) => nil)) ..))))))
   (at level 200, x1 closed binder, xn closed binder, E at level 0, S2 at level 0).
 
 Notation "'ATOMIC' 'TYPE' W 'OBJ' x 'INVS' E 'WITH' x1 , .. , xn 'PRE'  [ ] 'PROP' ( Px ; .. ; Py ) 'PARAMS' ( Lx ; .. ; Ly ) 'GLOBALS' ( Gx ; .. ; Gy ) 'SEP' ( S1x ; .. ; S1y ) '|' S2 'POST' [ tz ] 'EX' r : T , 'PROP' () 'LOCAL' ( LQx ; .. ; LQy ) 'SEP' ( SPx ; .. ; SPy ) '|' ( SQx ; .. ; SQy )" :=
   (mk_funspec (pair nil tz) cc_default ⊤ (atomic_spec_type W T)
    (atomic_spec_pre'(T := T) W
-      (OfeMor (rev_curry (tcurry (fun x1 => .. (tcurry (fun xn (_ : tuple_type tnil) => (cons Px%type .. (cons Py%type nil) ..))) ..))))
-      (OfeMor (rev_curry (tcurry (fun x1 => .. (tcurry (fun xn (_ : tuple_type tnil) => (cons Lx%type .. (cons Ly%type nil) ..))) ..))))
-      (OfeMor (rev_curry (tcurry (fun x1 => .. (tcurry (fun xn (_ : tuple_type tnil) => (cons Gx .. (cons Gy nil) ..))) ..))))
-      (OfeMor (rev_curry (tcurry (fun x1 => .. (tcurry (fun xn (_ : tuple_type tnil) => (cons S1x%I .. (cons S1y%I nil) ..))) ..))))
-      (OfeMor (rev_curry (tcurry (fun x1 => .. (tcurry (fun xn (_ : tuple_type tnil) x => S2)) ..))))
-      (OfeMor (rev_curry (tcurry (fun x1 => .. (tcurry (fun xn (_ : tuple_type tnil) => E)) ..))))
-      (OfeMor (rev_curry (tcurry (fun x1 => .. (tcurry (fun xn (_ : tuple_type tnil) x r => fold_right_sepcon (cons SQx%I .. (cons SQy%I nil) ..))) ..)))))
+      (OfeMor(ofe_mor_ne := _) (rev_curry (tcurry (fun x1 => .. (tcurry (fun xn (_ : tuple_type tnil) => (cons Px%type .. (cons Py%type nil) ..))) ..))))
+      (OfeMor(ofe_mor_ne := _) (rev_curry (tcurry (fun x1 => .. (tcurry (fun xn (_ : tuple_type tnil) => (cons Lx%type .. (cons Ly%type nil) ..))) ..))))
+      (OfeMor(ofe_mor_ne := _) (rev_curry (tcurry (fun x1 => .. (tcurry (fun xn (_ : tuple_type tnil) => (cons Gx .. (cons Gy nil) ..))) ..))))
+      (OfeMor(ofe_mor_ne := _) (rev_curry (tcurry (fun x1 => .. (tcurry (fun xn (_ : tuple_type tnil) => (cons S1x%I .. (cons S1y%I nil) ..))) ..))))
+      (OfeMor(ofe_mor_ne := _) (rev_curry (tcurry (fun x1 => .. (tcurry (fun xn (_ : tuple_type tnil) x => S2)) ..))))
+      (OfeMor(ofe_mor_ne := _) (rev_curry (tcurry (fun x1 => .. (tcurry (fun xn (_ : tuple_type tnil) => E)) ..))))
+      (OfeMor(ofe_mor_ne := _) (rev_curry (tcurry (fun x1 => .. (tcurry (fun xn (_ : tuple_type tnil) x r => fold_right_sepcon (cons SQx%I .. (cons SQy%I nil) ..))) ..)))))
   (atomic_spec_post' W
-      (OfeMor (rev_curry (tcurry (fun x1 => .. (tcurry (fun xn (_ : tuple_type tnil) r => (cons LQx%assert3 .. (cons LQy%assert3 nil) ..))) ..))))
-      (OfeMor (rev_curry (tcurry (fun x1 => .. (tcurry (fun xn (_ : tuple_type tnil) r => (cons SPx%assert3 .. (cons SPy%assert3 nil) ..))) ..))))))
+      (OfeMor(ofe_mor_ne := _) (rev_curry (tcurry (fun x1 => .. (tcurry (fun xn (_ : tuple_type tnil) r => (cons LQx%assert3 .. (cons LQy%assert3 nil) ..))) ..))))
+      (OfeMor(ofe_mor_ne := _) (rev_curry (tcurry (fun x1 => .. (tcurry (fun xn (_ : tuple_type tnil) r => (cons SPx%assert3 .. (cons SPy%assert3 nil) ..))) ..))))))
   (at level 200, x1 closed binder, xn closed binder, x at level 0, E at level 0, S2 at level 0, r at level 0, T at level 0).
 
 Notation "'ATOMIC' 'TYPE' W 'OBJ' x 'INVS' E 'WITH' x1 , .. , xn 'PRE'  [ ] 'PROP' ( Px ; .. ; Py ) 'PARAMS' ( Lx ; .. ; Ly ) 'GLOBALS' ( Gx ; .. ; Gy ) 'SEP' ( S1x ; .. ; S1y ) '|' S2 'POST' [ tz ] 'EX' r : T , 'PROP' () 'LOCAL' () 'SEP' ( SPx ; .. ; SPy ) '|' ( SQx ; .. ; SQy )" :=
   (mk_funspec (pair nil tz) cc_default ⊤ (atomic_spec_type W T)
    (atomic_spec_pre'(T := T) W
-      (OfeMor (rev_curry (tcurry (fun x1 => .. (tcurry (fun xn (_ : tuple_type tnil) => (cons Px%type .. (cons Py%type nil) ..))) ..))))
-      (OfeMor (rev_curry (tcurry (fun x1 => .. (tcurry (fun xn (_ : tuple_type tnil) => (cons Lx%type .. (cons Ly%type nil) ..))) ..))))
-      (OfeMor (rev_curry (tcurry (fun x1 => .. (tcurry (fun xn (_ : tuple_type tnil) => (cons Gx .. (cons Gy nil) ..))) ..))))
-      (OfeMor (rev_curry (tcurry (fun x1 => .. (tcurry (fun xn (_ : tuple_type tnil) => (cons S1x%I .. (cons S1y%I nil) ..))) ..))))
-      (OfeMor (rev_curry (tcurry (fun x1 => .. (tcurry (fun xn (_ : tuple_type tnil) x => S2)) ..))))
-      (OfeMor (rev_curry (tcurry (fun x1 => .. (tcurry (fun xn (_ : tuple_type tnil) => E)) ..))))
-      (OfeMor (rev_curry (tcurry (fun x1 => .. (tcurry (fun xn (_ : tuple_type tnil) x r => fold_right_sepcon (cons SQx%I .. (cons SQy%I nil) ..))) ..)))))
+      (OfeMor(ofe_mor_ne := _) (rev_curry (tcurry (fun x1 => .. (tcurry (fun xn (_ : tuple_type tnil) => (cons Px%type .. (cons Py%type nil) ..))) ..))))
+      (OfeMor(ofe_mor_ne := _) (rev_curry (tcurry (fun x1 => .. (tcurry (fun xn (_ : tuple_type tnil) => (cons Lx%type .. (cons Ly%type nil) ..))) ..))))
+      (OfeMor(ofe_mor_ne := _) (rev_curry (tcurry (fun x1 => .. (tcurry (fun xn (_ : tuple_type tnil) => (cons Gx .. (cons Gy nil) ..))) ..))))
+      (OfeMor(ofe_mor_ne := _) (rev_curry (tcurry (fun x1 => .. (tcurry (fun xn (_ : tuple_type tnil) => (cons S1x%I .. (cons S1y%I nil) ..))) ..))))
+      (OfeMor(ofe_mor_ne := _) (rev_curry (tcurry (fun x1 => .. (tcurry (fun xn (_ : tuple_type tnil) x => S2)) ..))))
+      (OfeMor(ofe_mor_ne := _) (rev_curry (tcurry (fun x1 => .. (tcurry (fun xn (_ : tuple_type tnil) => E)) ..))))
+      (OfeMor(ofe_mor_ne := _) (rev_curry (tcurry (fun x1 => .. (tcurry (fun xn (_ : tuple_type tnil) x r => fold_right_sepcon (cons SQx%I .. (cons SQy%I nil) ..))) ..)))))
   (atomic_spec_post' W
-      (OfeMor (rev_curry (tcurry (fun x1 => .. (tcurry (fun xn (_ : tuple_type tnil) r => nil)) ..))))
-      (OfeMor (rev_curry (tcurry (fun x1 => .. (tcurry (fun xn (_ : tuple_type tnil) r => (cons SPx%assert5%assert3 .. (cons SPy%assert5%assert3 nil) ..))) ..))))))
+      (OfeMor(ofe_mor_ne := _)(B := leibnizO (list localdef)) (rev_curry (tcurry (fun x1 => .. (tcurry (fun xn (_ : tuple_type tnil) r => nil)) ..))))
+      (OfeMor(ofe_mor_ne := _) (rev_curry (tcurry (fun x1 => .. (tcurry (fun xn (_ : tuple_type tnil) r => (cons SPx%assert5%assert3 .. (cons SPy%assert5%assert3 nil) ..))) ..))))))
   (at level 200, x1 closed binder, xn closed binder, x at level 0, E at level 0, S2 at level 0, r at level 0, T at level 0).
 
 Notation "'ATOMIC' 'TYPE' W 'OBJ' x 'INVS' E 'WITH' x1 , .. , xn 'PRE'  [ ] 'PROP' ( Px ; .. ; Py ) 'PARAMS ( Lx ; .. ; Ly ) 'GLOBALS' ( Gx ; .. ; Gy ) 'SEP' ( S1x ; .. ; S1y ) '|' S2 'POST' [ tz ] 'PROP' () 'LOCAL' ( LQx ; .. ; LQy ) 'SEP' ( SPx ; .. ; SPy ) '|' ( SQx ; .. ; SQy )" :=
   (mk_funspec (pair nil tz) cc_default ⊤ (atomic_spec_type0 W)
    (atomic_spec_pre0 W
-      (OfeMor (rev_curry (tcurry (fun x1 => .. (tcurry (fun xn (_ : tuple_type tnil) => (cons Px%type .. (cons Py%type nil) ..))) ..))))
-      (OfeMor (rev_curry (tcurry (fun x1 => .. (tcurry (fun xn (_ : tuple_type tnil) => (cons Lx%type .. (cons Ly%type nil) ..))) ..))))
-      (OfeMor (rev_curry (tcurry (fun x1 => .. (tcurry (fun xn (_ : tuple_type tnil) => (cons Gx .. (cons Gy nil) ..))) ..))))
-      (OfeMor (rev_curry (tcurry (fun x1 => .. (tcurry (fun xn (_ : tuple_type tnil) => (cons S1x%I .. (cons S1y%I nil) ..))) ..))))
-      (OfeMor (rev_curry (tcurry (fun x1 => .. (tcurry (fun xn (_ : tuple_type tnil) x => S2)) ..))))
-      (OfeMor (rev_curry (tcurry (fun x1 => .. (tcurry (fun xn (_ : tuple_type tnil) => E)) ..))))
-      (OfeMor (rev_curry (tcurry (fun x1 => .. (tcurry (fun xn (_ : tuple_type tnil) x _ => fold_right_sepcon (cons SQx%I .. (cons SQy%I nil) ..))) ..)))))
+      (OfeMor(ofe_mor_ne := _) (rev_curry (tcurry (fun x1 => .. (tcurry (fun xn (_ : tuple_type tnil) => (cons Px%type .. (cons Py%type nil) ..))) ..))))
+      (OfeMor(ofe_mor_ne := _) (rev_curry (tcurry (fun x1 => .. (tcurry (fun xn (_ : tuple_type tnil) => (cons Lx%type .. (cons Ly%type nil) ..))) ..))))
+      (OfeMor(ofe_mor_ne := _) (rev_curry (tcurry (fun x1 => .. (tcurry (fun xn (_ : tuple_type tnil) => (cons Gx .. (cons Gy nil) ..))) ..))))
+      (OfeMor(ofe_mor_ne := _) (rev_curry (tcurry (fun x1 => .. (tcurry (fun xn (_ : tuple_type tnil) => (cons S1x%I .. (cons S1y%I nil) ..))) ..))))
+      (OfeMor(ofe_mor_ne := _) (rev_curry (tcurry (fun x1 => .. (tcurry (fun xn (_ : tuple_type tnil) x => S2)) ..))))
+      (OfeMor(ofe_mor_ne := _) (rev_curry (tcurry (fun x1 => .. (tcurry (fun xn (_ : tuple_type tnil) => E)) ..))))
+      (OfeMor(ofe_mor_ne := _) (rev_curry (tcurry (fun x1 => .. (tcurry (fun xn (_ : tuple_type tnil) x _ => fold_right_sepcon (cons SQx%I .. (cons SQy%I nil) ..))) ..)))))
   (atomic_spec_post0 W
-      (OfeMor (rev_curry (tcurry (fun x1 => .. (tcurry (fun xn (_ : tuple_type tnil) => (cons LQx%assert3 .. (cons LQy%assert3 nil) ..))) ..))))
+      (OfeMor(ofe_mor_ne := _) (rev_curry (tcurry (fun x1 => .. (tcurry (fun xn (_ : tuple_type tnil) => (cons LQx%assert3 .. (cons LQy%assert3 nil) ..))) ..))))
       (rev_curry (tcurry (fun x1 => .. (tcurry (fun xn (_ : tuple_type tnil) => (cons SPx%assert3 .. (cons SPy%assert3 nil) ..))) ..)))))
   (at level 200, x1 closed binder, xn closed binder, x at level 0, E at level 0, S2 at level 0).
 
 Notation "'ATOMIC' 'TYPE' W 'OBJ' x 'INVS' E 'WITH' x1 , .. , xn 'PRE'  [ ] 'PROP' ( Px ; .. ; Py ) 'PARAMS' ( Lx ; .. ; Ly ) 'GLOBALS' ( Gx ; .. ; Gy ) 'SEP' ( S1x ; .. ; S1y ) '|' S2 'POST' [ tz ] 'PROP' () 'LOCAL' () 'SEP' ( SPx ; .. ; SPy ) '|' ( SQx ; .. ; SQy )" :=
   (mk_funspec (pair nil tz) cc_default ⊤ (atomic_spec_type0 W)
    (atomic_spec_pre0 W
-      (OfeMor (rev_curry (tcurry (fun x1 => .. (tcurry (fun xn (_ : tuple_type tnil) => (cons Px%type .. (cons Py%type nil) ..))) ..))))
-      (OfeMor (rev_curry (tcurry (fun x1 => .. (tcurry (fun xn (_ : tuple_type tnil) => (cons Lx%type .. (cons Ly%type nil) ..))) ..))))
-      (OfeMor (rev_curry (tcurry (fun x1 => .. (tcurry (fun xn (_ : tuple_type tnil) => (cons Gx .. (cons Gy nil) ..))) ..))))
-      (OfeMor (rev_curry (tcurry (fun x1 => .. (tcurry (fun xn (_ : tuple_type tnil) => (cons S1x%I .. (cons S1y%I nil) ..))) ..))))
-      (OfeMor (rev_curry (tcurry (fun x1 => .. (tcurry (fun xn (_ : tuple_type tnil) x => S2)) ..))))
-      (OfeMor (rev_curry (tcurry (fun x1 => .. (tcurry (fun xn (_ : tuple_type tnil) => E)) ..))))
-      (OfeMor (rev_curry (tcurry (fun x1 => .. (tcurry (fun xn (_ : tuple_type tnil) x _ => fold_right_sepcon (cons SQx%I .. (cons SQy%I nil) ..))) ..)))))
+      (OfeMor(ofe_mor_ne := _) (rev_curry (tcurry (fun x1 => .. (tcurry (fun xn (_ : tuple_type tnil) => (cons Px%type .. (cons Py%type nil) ..))) ..))))
+      (OfeMor(ofe_mor_ne := _) (rev_curry (tcurry (fun x1 => .. (tcurry (fun xn (_ : tuple_type tnil) => (cons Lx%type .. (cons Ly%type nil) ..))) ..))))
+      (OfeMor(ofe_mor_ne := _) (rev_curry (tcurry (fun x1 => .. (tcurry (fun xn (_ : tuple_type tnil) => (cons Gx .. (cons Gy nil) ..))) ..))))
+      (OfeMor(ofe_mor_ne := _) (rev_curry (tcurry (fun x1 => .. (tcurry (fun xn (_ : tuple_type tnil) => (cons S1x%I .. (cons S1y%I nil) ..))) ..))))
+      (OfeMor(ofe_mor_ne := _) (rev_curry (tcurry (fun x1 => .. (tcurry (fun xn (_ : tuple_type tnil) x => S2)) ..))))
+      (OfeMor(ofe_mor_ne := _) (rev_curry (tcurry (fun x1 => .. (tcurry (fun xn (_ : tuple_type tnil) => E)) ..))))
+      (OfeMor(ofe_mor_ne := _) (rev_curry (tcurry (fun x1 => .. (tcurry (fun xn (_ : tuple_type tnil) x _ => fold_right_sepcon (cons SQx%I .. (cons SQy%I nil) ..))) ..)))))
   (atomic_spec_post0 W
-      (OfeMor (rev_curry (tcurry (fun x1 => .. (tcurry (fun xn (_ : tuple_type tnil) => nil)) ..))))
-      (OfeMor (rev_curry (tcurry (fun x1 => .. (tcurry (fun xn (_ : tuple_type tnil) => (cons SPx%assert5%assert3 .. (cons SPy%assert5%assert3 nil) ..))) ..))))))
+      (OfeMor(ofe_mor_ne := _)(B := leibnizO (list localdef)) (rev_curry (tcurry (fun x1 => .. (tcurry (fun xn (_ : tuple_type tnil) => nil)) ..))))
+      (OfeMor(ofe_mor_ne := _) (rev_curry (tcurry (fun x1 => .. (tcurry (fun xn (_ : tuple_type tnil) => (cons SPx%assert5%assert3 .. (cons SPy%assert5%assert3 nil) ..))) ..))))))
   (at level 200, x1 closed binder, xn closed binder, x at level 0, E at level 0, S2 at level 0).
 
 Notation "'ATOMIC' 'TYPE' W 'OBJ' x 'INVS' E 'WITH' x1 , .. , xn 'PRE'  [ u , .. , v ] 'PROP' ( Px ; .. ; Py ) 'PARAMS' () 'GLOBALS' ( Gx ; .. ; Gy ) 'SEP' ( S1x ; .. ; S1y ) '|' S2 'POST' [ tz ] 'EX' r : T , 'PROP' () 'LOCAL' ( LQx ; .. ; LQy ) 'SEP' ( SPx ; .. ; SPy ) '|' ( SQx ; .. ; SQy )" :=
   (mk_funspec (pair (cons u%type .. (cons v%type nil) ..) tz) cc_default ⊤ (atomic_spec_type W T)
    (atomic_spec_pre'(T := T) W
-      (OfeMor (rev_curry (tcurry (fun x1 => .. (tcurry (fun xn (_ : tuple_type tnil) => (cons Px%type .. (cons Py%type nil) ..))) ..))))
-      (OfeMor (rev_curry (tcurry (fun x1 => .. (tcurry (fun xn (_ : tuple_type tnil) => nil)) ..))))
-      (OfeMor (rev_curry (tcurry (fun x1 => .. (tcurry (fun xn (_ : tuple_type tnil) => (cons Gx .. (cons Gy nil) ..))) ..))))
-      (OfeMor (rev_curry (tcurry (fun x1 => .. (tcurry (fun xn (_ : tuple_type tnil) => (cons S1x%I .. (cons S1y%I nil) ..))) ..))))
-      (OfeMor (rev_curry (tcurry (fun x1 => .. (tcurry (fun xn (_ : tuple_type tnil) x => S2)) ..))))
-      (OfeMor (rev_curry (tcurry (fun x1 => .. (tcurry (fun xn (_ : tuple_type tnil) => E)) ..))))
-      (OfeMor (rev_curry (tcurry (fun x1 => .. (tcurry (fun xn (_ : tuple_type tnil) x r => fold_right_sepcon (cons SQx%I .. (cons SQy%I nil) ..))) ..)))))
+      (OfeMor(ofe_mor_ne := _) (rev_curry (tcurry (fun x1 => .. (tcurry (fun xn (_ : tuple_type tnil) => (cons Px%type .. (cons Py%type nil) ..))) ..))))
+      (OfeMor(ofe_mor_ne := _) (rev_curry (tcurry (fun x1 => .. (tcurry (fun xn (_ : tuple_type tnil) => nil)) ..))))
+      (OfeMor(ofe_mor_ne := _) (rev_curry (tcurry (fun x1 => .. (tcurry (fun xn (_ : tuple_type tnil) => (cons Gx .. (cons Gy nil) ..))) ..))))
+      (OfeMor(ofe_mor_ne := _) (rev_curry (tcurry (fun x1 => .. (tcurry (fun xn (_ : tuple_type tnil) => (cons S1x%I .. (cons S1y%I nil) ..))) ..))))
+      (OfeMor(ofe_mor_ne := _) (rev_curry (tcurry (fun x1 => .. (tcurry (fun xn (_ : tuple_type tnil) x => S2)) ..))))
+      (OfeMor(ofe_mor_ne := _) (rev_curry (tcurry (fun x1 => .. (tcurry (fun xn (_ : tuple_type tnil) => E)) ..))))
+      (OfeMor(ofe_mor_ne := _) (rev_curry (tcurry (fun x1 => .. (tcurry (fun xn (_ : tuple_type tnil) x r => fold_right_sepcon (cons SQx%I .. (cons SQy%I nil) ..))) ..)))))
   (atomic_spec_post' W
-      (OfeMor (rev_curry (tcurry (fun x1 => .. (tcurry (fun xn (_ : tuple_type tnil) r => (cons LQx%assert3 .. (cons LQy%assert3 nil) ..))) ..))))
-      (OfeMor (rev_curry (tcurry (fun x1 => .. (tcurry (fun xn (_ : tuple_type tnil) r => (cons SPx%assert3 .. (cons SPy%assert3 nil) ..))) ..))))))
+      (OfeMor(ofe_mor_ne := _) (rev_curry (tcurry (fun x1 => .. (tcurry (fun xn (_ : tuple_type tnil) r => (cons LQx%assert3 .. (cons LQy%assert3 nil) ..))) ..))))
+      (OfeMor(ofe_mor_ne := _) (rev_curry (tcurry (fun x1 => .. (tcurry (fun xn (_ : tuple_type tnil) r => (cons SPx%assert3 .. (cons SPy%assert3 nil) ..))) ..))))))
   (at level 200, x1 closed binder, xn closed binder, x at level 0, E at level 0, S2 at level 0, r at level 0, T at level 0).
 
 Notation "'ATOMIC' 'TYPE' W 'OBJ' x 'INVS' E 'WITH' x1 , .. , xn 'PRE'  [ u , .. , v ] 'PROP' ( Px ; .. ; Py ) 'PARAMS' () 'GLOBALS' ( Gx ; .. ; Gy ) 'SEP' ( S1x ; .. ; S1y ) '|' S2 'POST' [ tz ] 'EX' r : T , 'PROP' () 'LOCAL' () 'SEP' ( SPx ; .. ; SPy ) '|' ( SQx ; .. ; SQy )" :=
   (mk_funspec (pair (cons u%type .. (cons v%type nil) ..) tz) cc_default ⊤ (atomic_spec_type W T)
    (atomic_spec_pre'(T := T) W
-      (OfeMor (rev_curry (tcurry (fun x1 => .. (tcurry (fun xn (_ : tuple_type tnil) => (cons Px%type .. (cons Py%type nil) ..))) ..))))
-      (OfeMor (rev_curry (tcurry (fun x1 => .. (tcurry (fun xn (_ : tuple_type tnil) => nil)) ..))))
-      (OfeMor (rev_curry (tcurry (fun x1 => .. (tcurry (fun xn (_ : tuple_type tnil) => (cons Gx .. (cons Gy nil) ..))) ..))))
-      (OfeMor (rev_curry (tcurry (fun x1 => .. (tcurry (fun xn (_ : tuple_type tnil) => (cons S1x%I .. (cons S1y%I nil) ..))) ..))))
-      (OfeMor (rev_curry (tcurry (fun x1 => .. (tcurry (fun xn (_ : tuple_type tnil) x => S2)) ..))))
-      (OfeMor (rev_curry (tcurry (fun x1 => .. (tcurry (fun xn (_ : tuple_type tnil) => E)) ..))))
-      (OfeMor (rev_curry (tcurry (fun x1 => .. (tcurry (fun xn (_ : tuple_type tnil) x r => fold_right_sepcon (cons SQx%I .. (cons SQy%I nil) ..))) ..)))))
+      (OfeMor(ofe_mor_ne := _) (rev_curry (tcurry (fun x1 => .. (tcurry (fun xn (_ : tuple_type tnil) => (cons Px%type .. (cons Py%type nil) ..))) ..))))
+      (OfeMor(ofe_mor_ne := _) (rev_curry (tcurry (fun x1 => .. (tcurry (fun xn (_ : tuple_type tnil) => nil)) ..))))
+      (OfeMor(ofe_mor_ne := _) (rev_curry (tcurry (fun x1 => .. (tcurry (fun xn (_ : tuple_type tnil) => (cons Gx .. (cons Gy nil) ..))) ..))))
+      (OfeMor(ofe_mor_ne := _) (rev_curry (tcurry (fun x1 => .. (tcurry (fun xn (_ : tuple_type tnil) => (cons S1x%I .. (cons S1y%I nil) ..))) ..))))
+      (OfeMor(ofe_mor_ne := _) (rev_curry (tcurry (fun x1 => .. (tcurry (fun xn (_ : tuple_type tnil) x => S2)) ..))))
+      (OfeMor(ofe_mor_ne := _) (rev_curry (tcurry (fun x1 => .. (tcurry (fun xn (_ : tuple_type tnil) => E)) ..))))
+      (OfeMor(ofe_mor_ne := _) (rev_curry (tcurry (fun x1 => .. (tcurry (fun xn (_ : tuple_type tnil) x r => fold_right_sepcon (cons SQx%I .. (cons SQy%I nil) ..))) ..)))))
   (atomic_spec_post' W
-      (OfeMor (rev_curry (tcurry (fun x1 => .. (tcurry (fun xn (_ : tuple_type tnil) r => nil)) ..))))
-      (OfeMor (rev_curry (tcurry (fun x1 => .. (tcurry (fun xn (_ : tuple_type tnil) r => (cons SPx%assert5%assert3 .. (cons SPy%assert5%assert3 nil) ..))) ..))))))
+      (OfeMor(ofe_mor_ne := _)(B := leibnizO (list localdef)) (rev_curry (tcurry (fun x1 => .. (tcurry (fun xn (_ : tuple_type tnil) r => nil)) ..))))
+      (OfeMor(ofe_mor_ne := _) (rev_curry (tcurry (fun x1 => .. (tcurry (fun xn (_ : tuple_type tnil) r => (cons SPx%assert5%assert3 .. (cons SPy%assert5%assert3 nil) ..))) ..))))))
   (at level 200, x1 closed binder, xn closed binder, x at level 0, E at level 0, S2 at level 0, r at level 0, T at level 0).
 
 Notation "'ATOMIC' 'TYPE' W 'OBJ' x 'INVS' E 'WITH' x1 , .. , xn 'PRE'  [ u , .. , v ] 'PROP' ( Px ; .. ; Py ) 'PARAMS' () 'GLOBALS' ( Gx ; .. ; Gy ) 'SEP' ( S1x ; .. ; S1y ) '|' S2 'POST' [ tz ] 'PROP' () 'LOCAL' ( LQx ; .. ; LQy ) 'SEP' ( SPx ; .. ; SPy ) '|' ( SQx ; .. ; SQy )" :=
   (mk_funspec (pair (cons u%type .. (cons v%type nil) ..) tz) cc_default ⊤ (atomic_spec_type0 W)
    (atomic_spec_pre0 W
-      (OfeMor (rev_curry (tcurry (fun x1 => .. (tcurry (fun xn (_ : tuple_type tnil) => (cons Px%type .. (cons Py%type nil) ..))) ..))))
-      (OfeMor (rev_curry (tcurry (fun x1 => .. (tcurry (fun xn (_ : tuple_type tnil) => nil)) ..))))
-      (OfeMor (rev_curry (tcurry (fun x1 => .. (tcurry (fun xn (_ : tuple_type tnil) => (cons Gx .. (cons Gy nil) ..))) ..))))
-      (OfeMor (rev_curry (tcurry (fun x1 => .. (tcurry (fun xn (_ : tuple_type tnil) => (cons S1x%I .. (cons S1y%I nil) ..))) ..))))
-      (OfeMor (rev_curry (tcurry (fun x1 => .. (tcurry (fun xn (_ : tuple_type tnil) x => S2)) ..))))
-      (OfeMor (rev_curry (tcurry (fun x1 => .. (tcurry (fun xn (_ : tuple_type tnil) => E)) ..))))
-      (OfeMor (rev_curry (tcurry (fun x1 => .. (tcurry (fun xn (_ : tuple_type tnil) x _ => fold_right_sepcon (cons SQx%I .. (cons SQy%I nil) ..))) ..)))))
+      (OfeMor(ofe_mor_ne := _) (rev_curry (tcurry (fun x1 => .. (tcurry (fun xn (_ : tuple_type tnil) => (cons Px%type .. (cons Py%type nil) ..))) ..))))
+      (OfeMor(ofe_mor_ne := _) (rev_curry (tcurry (fun x1 => .. (tcurry (fun xn (_ : tuple_type tnil) => nil)) ..))))
+      (OfeMor(ofe_mor_ne := _) (rev_curry (tcurry (fun x1 => .. (tcurry (fun xn (_ : tuple_type tnil) => (cons Gx .. (cons Gy nil) ..))) ..))))
+      (OfeMor(ofe_mor_ne := _) (rev_curry (tcurry (fun x1 => .. (tcurry (fun xn (_ : tuple_type tnil) => (cons S1x%I .. (cons S1y%I nil) ..))) ..))))
+      (OfeMor(ofe_mor_ne := _) (rev_curry (tcurry (fun x1 => .. (tcurry (fun xn (_ : tuple_type tnil) x => S2)) ..))))
+      (OfeMor(ofe_mor_ne := _) (rev_curry (tcurry (fun x1 => .. (tcurry (fun xn (_ : tuple_type tnil) => E)) ..))))
+      (OfeMor(ofe_mor_ne := _) (rev_curry (tcurry (fun x1 => .. (tcurry (fun xn (_ : tuple_type tnil) x _ => fold_right_sepcon (cons SQx%I .. (cons SQy%I nil) ..))) ..)))))
   (atomic_spec_post0 W
-      (OfeMor (rev_curry (tcurry (fun x1 => .. (tcurry (fun xn (_ : tuple_type tnil) => (cons LQx%assert3 .. (cons LQy%assert3 nil) ..))) ..))))
-      (OfeMor (rev_curry (tcurry (fun x1 => .. (tcurry (fun xn (_ : tuple_type tnil) => (cons SPx%assert3 .. (cons SPy%assert3 nil) ..))) ..))))))
+      (OfeMor(ofe_mor_ne := _) (rev_curry (tcurry (fun x1 => .. (tcurry (fun xn (_ : tuple_type tnil) => (cons LQx%assert3 .. (cons LQy%assert3 nil) ..))) ..))))
+      (OfeMor(ofe_mor_ne := _) (rev_curry (tcurry (fun x1 => .. (tcurry (fun xn (_ : tuple_type tnil) => (cons SPx%assert3 .. (cons SPy%assert3 nil) ..))) ..))))))
   (at level 200, x1 closed binder, xn closed binder, x at level 0, E at level 0, S2 at level 0).
 
 Notation "'ATOMIC' 'TYPE' W 'OBJ' x 'INVS' E 'WITH' x1 , .. , xn 'PRE'  [ u , .. , v ] 'PROP' ( Px ; .. ; Py ) 'PARAMS' () 'GLOBALS' ( Gx ; .. ; Gy ) 'SEP' ( S1x ; .. ; S1y ) '|' S2 'POST' [ tz ] 'PROP' () 'LOCAL' () 'SEP' ( SPx ; .. ; SPy ) '|' ( SQx ; .. ; SQy )" :=
   (mk_funspec (pair (cons u%type .. (cons v%type nil) ..) tz) cc_default ⊤ (atomic_spec_type0 W)
    (atomic_spec_pre0 W
-      (OfeMor (rev_curry (tcurry (fun x1 => .. (tcurry (fun xn (_ : tuple_type tnil) => (cons Px%type .. (cons Py%type nil) ..))) ..))))
-      (OfeMor (rev_curry (tcurry (fun x1 => .. (tcurry (fun xn (_ : tuple_type tnil) => nil)) ..))))
-      (OfeMor (rev_curry (tcurry (fun x1 => .. (tcurry (fun xn (_ : tuple_type tnil) => (cons Gx .. (cons Gy nil) ..))) ..))))
-      (OfeMor (rev_curry (tcurry (fun x1 => .. (tcurry (fun xn (_ : tuple_type tnil) => (cons S1x%I .. (cons S1y%I nil) ..))) ..))))
-      (OfeMor (rev_curry (tcurry (fun x1 => .. (tcurry (fun xn (_ : tuple_type tnil) x => S2)) ..))))       (OfeMor (rev_curry (tcurry (fun x1 => .. (tcurry (fun xn (_ : tuple_type tnil) => E)) ..))))
-      (OfeMor (rev_curry (tcurry (fun x1 => .. (tcurry (fun xn (_ : tuple_type tnil) x _ => fold_right_sepcon (cons SQx%I .. (cons SQy%I nil) ..))) ..)))))
+      (OfeMor(ofe_mor_ne := _) (rev_curry (tcurry (fun x1 => .. (tcurry (fun xn (_ : tuple_type tnil) => (cons Px%type .. (cons Py%type nil) ..))) ..))))
+      (OfeMor(ofe_mor_ne := _) (rev_curry (tcurry (fun x1 => .. (tcurry (fun xn (_ : tuple_type tnil) => nil)) ..))))
+      (OfeMor(ofe_mor_ne := _) (rev_curry (tcurry (fun x1 => .. (tcurry (fun xn (_ : tuple_type tnil) => (cons Gx .. (cons Gy nil) ..))) ..))))
+      (OfeMor(ofe_mor_ne := _) (rev_curry (tcurry (fun x1 => .. (tcurry (fun xn (_ : tuple_type tnil) => (cons S1x%I .. (cons S1y%I nil) ..))) ..))))
+      (OfeMor(ofe_mor_ne := _) (rev_curry (tcurry (fun x1 => .. (tcurry (fun xn (_ : tuple_type tnil) x => S2)) ..))))       (OfeMor(ofe_mor_ne := _) (rev_curry (tcurry (fun x1 => .. (tcurry (fun xn (_ : tuple_type tnil) => E)) ..))))
+      (OfeMor(ofe_mor_ne := _) (rev_curry (tcurry (fun x1 => .. (tcurry (fun xn (_ : tuple_type tnil) x _ => fold_right_sepcon (cons SQx%I .. (cons SQy%I nil) ..))) ..)))))
   (atomic_spec_post0 W
-      (OfeMor (rev_curry (tcurry (fun x1 => .. (tcurry (fun xn (_ : tuple_type tnil) => nil)) ..))))
-      (OfeMor (rev_curry (tcurry (fun x1 => .. (tcurry (fun xn (_ : tuple_type tnil) => (cons SPx%assert5%assert3 .. (cons SPy%assert5%assert3 nil) ..))) ..))))))
+      (OfeMor(ofe_mor_ne := _)(B := leibnizO (list localdef)) (rev_curry (tcurry (fun x1 => .. (tcurry (fun xn (_ : tuple_type tnil) => nil)) ..))))
+      (OfeMor(ofe_mor_ne := _) (rev_curry (tcurry (fun x1 => .. (tcurry (fun xn (_ : tuple_type tnil) => (cons SPx%assert5%assert3 .. (cons SPy%assert5%assert3 nil) ..))) ..))))))
   (at level 200, x1 closed binder, xn closed binder, x at level 0, E at level 0, S2 at level 0).
 
 Notation "'ATOMIC' 'TYPE' W 'OBJ' x 'INVS' E 'WITH' x1 , .. , xn 'PRE'  [ ] 'PROP' ( Px ; .. ; Py ) 'PARAMS' () 'GLOBALS' ( Gx ; .. ; Gy ) 'SEP' ( S1x ; .. ; S1y ) '|' S2 'POST' [ tz ] 'EX' r : T , 'PROP' () 'LOCAL' ( LQx ; .. ; LQy ) 'SEP' ( SPx ; .. ; SPy ) '|' ( SQx ; .. ; SQy )" :=
   (mk_funspec (pair nil tz) cc_default ⊤ (atomic_spec_type W T)
    (atomic_spec_pre' (T := T) W
-      (OfeMor (rev_curry (tcurry (fun x1 => .. (tcurry (fun xn (_ : tuple_type tnil) => (cons Px%type .. (cons Py%type nil) ..))) ..))))
-      (OfeMor (rev_curry (tcurry (fun x1 => .. (tcurry (fun xn (_ : tuple_type tnil) => nil)) ..))))
-      (OfeMor (rev_curry (tcurry (fun x1 => .. (tcurry (fun xn (_ : tuple_type tnil) => (cons Gx .. (cons Gy nil) ..))) ..))))
-      (OfeMor (rev_curry (tcurry (fun x1 => .. (tcurry (fun xn (_ : tuple_type tnil) => (cons S1x%I .. (cons S1y%I nil) ..))) ..))))
-      (OfeMor (rev_curry (tcurry (fun x1 => .. (tcurry (fun xn (_ : tuple_type tnil) x => S2)) ..))))
-      (OfeMor (rev_curry (tcurry (fun x1 => .. (tcurry (fun xn (_ : tuple_type tnil) => E)) ..))))
-      (OfeMor (rev_curry (tcurry (fun x1 => .. (tcurry (fun xn (_ : tuple_type tnil) x r => fold_right_sepcon (cons SQx%I .. (cons SQy%I nil) ..))) ..)))))
+      (OfeMor(ofe_mor_ne := _) (rev_curry (tcurry (fun x1 => .. (tcurry (fun xn (_ : tuple_type tnil) => (cons Px%type .. (cons Py%type nil) ..))) ..))))
+      (OfeMor(ofe_mor_ne := _) (rev_curry (tcurry (fun x1 => .. (tcurry (fun xn (_ : tuple_type tnil) => nil)) ..))))
+      (OfeMor(ofe_mor_ne := _) (rev_curry (tcurry (fun x1 => .. (tcurry (fun xn (_ : tuple_type tnil) => (cons Gx .. (cons Gy nil) ..))) ..))))
+      (OfeMor(ofe_mor_ne := _) (rev_curry (tcurry (fun x1 => .. (tcurry (fun xn (_ : tuple_type tnil) => (cons S1x%I .. (cons S1y%I nil) ..))) ..))))
+      (OfeMor(ofe_mor_ne := _) (rev_curry (tcurry (fun x1 => .. (tcurry (fun xn (_ : tuple_type tnil) x => S2)) ..))))
+      (OfeMor(ofe_mor_ne := _) (rev_curry (tcurry (fun x1 => .. (tcurry (fun xn (_ : tuple_type tnil) => E)) ..))))
+      (OfeMor(ofe_mor_ne := _) (rev_curry (tcurry (fun x1 => .. (tcurry (fun xn (_ : tuple_type tnil) x r => fold_right_sepcon (cons SQx%I .. (cons SQy%I nil) ..))) ..)))))
   (atomic_spec_post' W
-      (OfeMor (rev_curry (tcurry (fun x1 => .. (tcurry (fun xn (_ : tuple_type tnil) r => (cons LQx%assert3 .. (cons LQy%assert3 nil) ..))) ..))))
-      (OfeMor (rev_curry (tcurry (fun x1 => .. (tcurry (fun xn (_ : tuple_type tnil) r => (cons SPx%assert3 .. (cons SPy%assert3 nil) ..))) ..))))))
+      (OfeMor(ofe_mor_ne := _) (rev_curry (tcurry (fun x1 => .. (tcurry (fun xn (_ : tuple_type tnil) r => (cons LQx%assert3 .. (cons LQy%assert3 nil) ..))) ..))))
+      (OfeMor(ofe_mor_ne := _) (rev_curry (tcurry (fun x1 => .. (tcurry (fun xn (_ : tuple_type tnil) r => (cons SPx%assert3 .. (cons SPy%assert3 nil) ..))) ..))))))
   (at level 200, x1 closed binder, xn closed binder, x at level 0, E at level 0, S2 at level 0, r at level 0, T at level 0).
 
 Notation "'ATOMIC' 'TYPE' W 'OBJ' x 'INVS' E 'WITH' x1 , .. , xn 'PRE'  [ ] 'PROP' () 'PARAMS' () 'GLOBALS' ( Gx ; .. ; Gy ) 'SEP' () '|' S2 'POST' [ tz ] 'EX' r : T , 'PROP' () 'LOCAL' ( LQx ; .. ; LQy ) 'SEP' () '|' ( SQx ; .. ; SQy )" :=
   (mk_funspec (pair nil tz) cc_default ⊤ (atomic_spec_type W T)
    (atomic_spec_pre' (T := T) W
-      (OfeMor (rev_curry (tcurry (fun x1 => .. (tcurry (fun xn (_ : tuple_type tnil) => nil)) ..))))
-      (OfeMor (rev_curry (tcurry (fun x1 => .. (tcurry (fun xn (_ : tuple_type tnil) => nil)) ..))))
-      (OfeMor (rev_curry (tcurry (fun x1 => .. (tcurry (fun xn (_ : tuple_type tnil) => (cons Gx .. (cons Gy nil) ..))) ..))))
-      (OfeMor (rev_curry (tcurry (fun x1 => .. (tcurry (fun xn (_ : tuple_type tnil) => nil)) ..))))
-      (OfeMor (rev_curry (tcurry (fun x1 => .. (tcurry (fun xn (_ : tuple_type tnil) x => S2)) ..))))
-      (OfeMor (rev_curry (tcurry (fun x1 => .. (tcurry (fun xn (_ : tuple_type tnil) => E)) ..))))
-      (OfeMor (rev_curry (tcurry (fun x1 => .. (tcurry (fun xn (_ : tuple_type tnil) x r => fold_right_sepcon (cons SQx%I .. (cons SQy%I nil) ..))) ..)))))
+      (OfeMor(ofe_mor_ne := _) (rev_curry (tcurry (fun x1 => .. (tcurry (fun xn (_ : tuple_type tnil) => nil)) ..))))
+      (OfeMor(ofe_mor_ne := _) (rev_curry (tcurry (fun x1 => .. (tcurry (fun xn (_ : tuple_type tnil) => nil)) ..))))
+      (OfeMor(ofe_mor_ne := _) (rev_curry (tcurry (fun x1 => .. (tcurry (fun xn (_ : tuple_type tnil) => (cons Gx .. (cons Gy nil) ..))) ..))))
+      (OfeMor(ofe_mor_ne := _) (rev_curry (tcurry (fun x1 => .. (tcurry (fun xn (_ : tuple_type tnil) => nil)) ..))))
+      (OfeMor(ofe_mor_ne := _) (rev_curry (tcurry (fun x1 => .. (tcurry (fun xn (_ : tuple_type tnil) x => S2)) ..))))
+      (OfeMor(ofe_mor_ne := _) (rev_curry (tcurry (fun x1 => .. (tcurry (fun xn (_ : tuple_type tnil) => E)) ..))))
+      (OfeMor(ofe_mor_ne := _) (rev_curry (tcurry (fun x1 => .. (tcurry (fun xn (_ : tuple_type tnil) x r => fold_right_sepcon (cons SQx%I .. (cons SQy%I nil) ..))) ..)))))
   (atomic_spec_post' W
-      (OfeMor (rev_curry (tcurry (fun x1 => .. (tcurry (fun xn (_ : tuple_type tnil) r => (cons LQx%assert3 .. (cons LQy%assert3 nil) ..))) ..))))
-      (OfeMor (rev_curry (tcurry (fun x1 => .. (tcurry (fun xn (_ : tuple_type tnil) r => nil)) ..))))))
+      (OfeMor(ofe_mor_ne := _) (rev_curry (tcurry (fun x1 => .. (tcurry (fun xn (_ : tuple_type tnil) r => (cons LQx%assert3 .. (cons LQy%assert3 nil) ..))) ..))))
+      (OfeMor(ofe_mor_ne := _)(B := list mpred) (rev_curry (tcurry (fun x1 => .. (tcurry (fun xn (_ : tuple_type tnil) r => nil)) ..))))))
   (at level 200, x1 closed binder, xn closed binder, x at level 0, E at level 0, S2 at level 0, r at level 0, T at level 0).
 
 Notation "'ATOMIC' 'TYPE' W 'OBJ' x 'INVS' E 'WITH' x1 , .. , xn 'PRE'  [ ] 'PROP' ( Px ; .. ; Py ) 'PARAMS' () 'GLOBALS' ( Gx ; .. ; Gy ) 'SEP' ( S1x ; .. ; S1y ) '|' S2 'POST' [ tz ] 'EX' r : T , 'PROP' () 'LOCAL' () 'SEP' ( SPx ; .. ; SPy ) '|' ( SQx ; .. ; SQy )" :=
   (mk_funspec (pair nil tz) cc_default ⊤ (atomic_spec_type W T)
    (atomic_spec_pre' (T := T) W
-      (OfeMor (rev_curry (tcurry (fun x1 => .. (tcurry (fun xn (_ : tuple_type tnil) => (cons Px%type .. (cons Py%type nil) ..))) ..))))
-      (OfeMor (rev_curry (tcurry (fun x1 => .. (tcurry (fun xn (_ : tuple_type tnil) => nil)) ..))))
-      (OfeMor (rev_curry (tcurry (fun x1 => .. (tcurry (fun xn (_ : tuple_type tnil) => (cons Gx .. (cons Gy nil) ..))) ..))))
-      (OfeMor (rev_curry (tcurry (fun x1 => .. (tcurry (fun xn (_ : tuple_type tnil) => (cons S1x%I .. (cons S1y%I nil) ..))) ..))))
-      (OfeMor (rev_curry (tcurry (fun x1 => .. (tcurry (fun xn (_ : tuple_type tnil) x => S2)) ..))))
-      (OfeMor (rev_curry (tcurry (fun x1 => .. (tcurry (fun xn (_ : tuple_type tnil) => E)) ..))))
-      (OfeMor (rev_curry (tcurry (fun x1 => .. (tcurry (fun xn (_ : tuple_type tnil) x r => fold_right_sepcon (cons SQx%I .. (cons SQy%I nil) ..))) ..)))))
+      (OfeMor(ofe_mor_ne := _) (rev_curry (tcurry (fun x1 => .. (tcurry (fun xn (_ : tuple_type tnil) => (cons Px%type .. (cons Py%type nil) ..))) ..))))
+      (OfeMor(ofe_mor_ne := _) (rev_curry (tcurry (fun x1 => .. (tcurry (fun xn (_ : tuple_type tnil) => nil)) ..))))
+      (OfeMor(ofe_mor_ne := _) (rev_curry (tcurry (fun x1 => .. (tcurry (fun xn (_ : tuple_type tnil) => (cons Gx .. (cons Gy nil) ..))) ..))))
+      (OfeMor(ofe_mor_ne := _) (rev_curry (tcurry (fun x1 => .. (tcurry (fun xn (_ : tuple_type tnil) => (cons S1x%I .. (cons S1y%I nil) ..))) ..))))
+      (OfeMor(ofe_mor_ne := _) (rev_curry (tcurry (fun x1 => .. (tcurry (fun xn (_ : tuple_type tnil) x => S2)) ..))))
+      (OfeMor(ofe_mor_ne := _) (rev_curry (tcurry (fun x1 => .. (tcurry (fun xn (_ : tuple_type tnil) => E)) ..))))
+      (OfeMor(ofe_mor_ne := _) (rev_curry (tcurry (fun x1 => .. (tcurry (fun xn (_ : tuple_type tnil) x r => fold_right_sepcon (cons SQx%I .. (cons SQy%I nil) ..))) ..)))))
   (atomic_spec_post' W
-      (OfeMor (rev_curry (tcurry (fun x1 => .. (tcurry (fun xn (_ : tuple_type tnil) r => nil)) ..))))
-      (OfeMor (rev_curry (tcurry (fun x1 => .. (tcurry (fun xn (_ : tuple_type tnil) r => (cons SPx%assert5%assert3 .. (cons SPy%assert5%assert3 nil) ..))) ..))))))
+      (OfeMor(ofe_mor_ne := _)(B := leibnizO (list localdef)) (rev_curry (tcurry (fun x1 => .. (tcurry (fun xn (_ : tuple_type tnil) r => nil)) ..))))
+      (OfeMor(ofe_mor_ne := _) (rev_curry (tcurry (fun x1 => .. (tcurry (fun xn (_ : tuple_type tnil) r => (cons SPx%assert5%assert3 .. (cons SPy%assert5%assert3 nil) ..))) ..))))))
   (at level 200, x1 closed binder, xn closed binder, x at level 0, E at level 0, S2 at level 0, r at level 0, T at level 0).
 
 Notation "'ATOMIC' 'TYPE' W 'OBJ' x 'INVS' E 'WITH' x1 , .. , xn 'PRE'  [ ] 'PROP' ( Px ; .. ; Py ) 'PARAMS' () 'GLOBALS' ( Gx ; .. ; Gy ) 'SEP' ( S1x ; .. ; S1y ) '|' S2 'POST' [ tz ] 'PROP' () 'LOCAL' ( LQx ; .. ; LQy ) 'SEP' ( SPx ; .. ; SPy ) '|' ( SQx ; .. ; SQy )" :=
   (mk_funspec (pair nil tz) cc_default ⊤ (atomic_spec_type0 W)
    (atomic_spec_pre0 W
-      (OfeMor (rev_curry (tcurry (fun x1 => .. (tcurry (fun xn (_ : tuple_type tnil) => (cons Px%type .. (cons Py%type nil) ..))) ..))))
-      (OfeMor (rev_curry (tcurry (fun x1 => .. (tcurry (fun xn (_ : tuple_type tnil) => nil)) ..))))
-      (OfeMor (rev_curry (tcurry (fun x1 => .. (tcurry (fun xn (_ : tuple_type tnil) => (cons Gx .. (cons Gy nil) ..))) ..))))
-      (OfeMor (rev_curry (tcurry (fun x1 => .. (tcurry (fun xn (_ : tuple_type tnil) => (cons S1x%I .. (cons S1y%I nil) ..))) ..))))
-      (OfeMor (rev_curry (tcurry (fun x1 => .. (tcurry (fun xn (_ : tuple_type tnil) x => S2)) ..))))
-      (OfeMor (rev_curry (tcurry (fun x1 => .. (tcurry (fun xn (_ : tuple_type tnil) => E)) ..))))
-      (OfeMor (rev_curry (tcurry (fun x1 => .. (tcurry (fun xn (_ : tuple_type tnil) x _ => fold_right_sepcon (cons SQx%I .. (cons SQy%I nil) ..))) ..)))))
+      (OfeMor(ofe_mor_ne := _) (rev_curry (tcurry (fun x1 => .. (tcurry (fun xn (_ : tuple_type tnil) => (cons Px%type .. (cons Py%type nil) ..))) ..))))
+      (OfeMor(ofe_mor_ne := _) (rev_curry (tcurry (fun x1 => .. (tcurry (fun xn (_ : tuple_type tnil) => nil)) ..))))
+      (OfeMor(ofe_mor_ne := _) (rev_curry (tcurry (fun x1 => .. (tcurry (fun xn (_ : tuple_type tnil) => (cons Gx .. (cons Gy nil) ..))) ..))))
+      (OfeMor(ofe_mor_ne := _) (rev_curry (tcurry (fun x1 => .. (tcurry (fun xn (_ : tuple_type tnil) => (cons S1x%I .. (cons S1y%I nil) ..))) ..))))
+      (OfeMor(ofe_mor_ne := _) (rev_curry (tcurry (fun x1 => .. (tcurry (fun xn (_ : tuple_type tnil) x => S2)) ..))))
+      (OfeMor(ofe_mor_ne := _) (rev_curry (tcurry (fun x1 => .. (tcurry (fun xn (_ : tuple_type tnil) => E)) ..))))
+      (OfeMor(ofe_mor_ne := _) (rev_curry (tcurry (fun x1 => .. (tcurry (fun xn (_ : tuple_type tnil) x _ => fold_right_sepcon (cons SQx%I .. (cons SQy%I nil) ..))) ..)))))
   (atomic_spec_post0 W
-      (OfeMor (rev_curry (tcurry (fun x1 => .. (tcurry (fun xn (_ : tuple_type tnil) => (cons LQx%assert3 .. (cons LQy%assert3 nil) ..))) ..))))
-      (OfeMor (rev_curry (tcurry (fun x1 => .. (tcurry (fun xn (_ : tuple_type tnil) => (cons SPx%assert3 .. (cons SPy%assert3 nil) ..))) ..))))))
+      (OfeMor(ofe_mor_ne := _) (rev_curry (tcurry (fun x1 => .. (tcurry (fun xn (_ : tuple_type tnil) => (cons LQx%assert3 .. (cons LQy%assert3 nil) ..))) ..))))
+      (OfeMor(ofe_mor_ne := _) (rev_curry (tcurry (fun x1 => .. (tcurry (fun xn (_ : tuple_type tnil) => (cons SPx%assert3 .. (cons SPy%assert3 nil) ..))) ..))))))
   (at level 200, x1 closed binder, xn closed binder, x at level 0, E at level 0, S2 at level 0).
 
 Notation "'ATOMIC' 'TYPE' W 'OBJ' x 'INVS' E 'WITH' x1 , .. , xn 'PRE'  [ ] 'PROP' ( Px ; .. ; Py ) 'PARAMS' () 'GLOBALS' ( Gx ; .. ; Gy ) 'SEP' ( S1x ; .. ; S1y ) '|' S2 'POST' [ tz ] 'PROP' () 'LOCAL' () 'SEP' ( SPx ; .. ; SPy ) '|' ( SQx ; .. ; SQy )" :=
   (mk_funspec (pair nil tz) cc_default ⊤ (atomic_spec_type0 W)
    (atomic_spec_pre0 W
-      (OfeMor (rev_curry (tcurry (fun x1 => .. (tcurry (fun xn (_ : tuple_type tnil) => (cons Px%type .. (cons Py%type nil) ..))) ..))))
-      (OfeMor (rev_curry (tcurry (fun x1 => .. (tcurry (fun xn (_ : tuple_type tnil) => nil)) ..))))
-      (OfeMor (rev_curry (tcurry (fun x1 => .. (tcurry (fun xn (_ : tuple_type tnil) => (cons Gx .. (cons Gy nil) ..))) ..))))
-      (OfeMor (rev_curry (tcurry (fun x1 => .. (tcurry (fun xn (_ : tuple_type tnil) => (cons S1x%I .. (cons S1y%I nil) ..))) ..))))
-      (OfeMor (rev_curry (tcurry (fun x1 => .. (tcurry (fun xn (_ : tuple_type tnil) x => S2)) ..))))
-      (OfeMor (rev_curry (tcurry (fun x1 => .. (tcurry (fun xn (_ : tuple_type tnil) => E)) ..))))
-      (OfeMor (rev_curry (tcurry (fun x1 => .. (tcurry (fun xn (_ : tuple_type tnil) x _ => fold_right_sepcon (cons SQx%I .. (cons SQy%I nil) ..))) ..)))))
+      (OfeMor(ofe_mor_ne := _) (rev_curry (tcurry (fun x1 => .. (tcurry (fun xn (_ : tuple_type tnil) => (cons Px%type .. (cons Py%type nil) ..))) ..))))
+      (OfeMor(ofe_mor_ne := _) (rev_curry (tcurry (fun x1 => .. (tcurry (fun xn (_ : tuple_type tnil) => nil)) ..))))
+      (OfeMor(ofe_mor_ne := _) (rev_curry (tcurry (fun x1 => .. (tcurry (fun xn (_ : tuple_type tnil) => (cons Gx .. (cons Gy nil) ..))) ..))))
+      (OfeMor(ofe_mor_ne := _) (rev_curry (tcurry (fun x1 => .. (tcurry (fun xn (_ : tuple_type tnil) => (cons S1x%I .. (cons S1y%I nil) ..))) ..))))
+      (OfeMor(ofe_mor_ne := _) (rev_curry (tcurry (fun x1 => .. (tcurry (fun xn (_ : tuple_type tnil) x => S2)) ..))))
+      (OfeMor(ofe_mor_ne := _) (rev_curry (tcurry (fun x1 => .. (tcurry (fun xn (_ : tuple_type tnil) => E)) ..))))
+      (OfeMor(ofe_mor_ne := _) (rev_curry (tcurry (fun x1 => .. (tcurry (fun xn (_ : tuple_type tnil) x _ => fold_right_sepcon (cons SQx%I .. (cons SQy%I nil) ..))) ..)))))
   (atomic_spec_post0 W
-      (OfeMor (rev_curry (tcurry (fun x1 => .. (tcurry (fun xn (_ : tuple_type tnil) => nil)) ..))))
-      (OfeMor (rev_curry (tcurry (fun x1 => .. (tcurry (fun xn (_ : tuple_type tnil) => (cons SPx%assert5%assert3 .. (cons SPy%assert5%assert3 nil) ..))) ..))))))
+      (OfeMor(ofe_mor_ne := _)(B := leibnizO (list localdef)) (rev_curry (tcurry (fun x1 => .. (tcurry (fun xn (_ : tuple_type tnil) => nil)) ..))))
+      (OfeMor(ofe_mor_ne := _) (rev_curry (tcurry (fun x1 => .. (tcurry (fun xn (_ : tuple_type tnil) => (cons SPx%assert5%assert3 .. (cons SPy%assert5%assert3 nil) ..))) ..))))))
   (at level 200, x1 closed binder, xn closed binder, x at level 0, E at level 0, S2 at level 0).
 
 Notation "'ATOMIC' 'TYPE' W 'OBJ' x 'INVS' E 'WITH' x1 , .. , xn 'PRE'  [ ] 'PROP' () 'PARAMS' () 'GLOBALS' ( Gx ; .. ; Gy ) 'SEP' () '|' S2 'POST' [ tz ] 'PROP' () 'LOCAL' ( LQx ; .. ; LQy ) 'SEP' () '|' ( SQx ; .. ; SQy )" :=
   (mk_funspec (pair nil tz) cc_default ⊤ (atomic_spec_type0 W)
    (atomic_spec_pre0 W
-      (OfeMor (rev_curry (tcurry (fun x1 => .. (tcurry (fun xn (_ : tuple_type tnil) => nil)) ..))))
-      (OfeMor (rev_curry (tcurry (fun x1 => .. (tcurry (fun xn (_ : tuple_type tnil) => nil)) ..))))
-      (OfeMor (rev_curry (tcurry (fun x1 => .. (tcurry (fun xn (_ : tuple_type tnil) => (cons Gx .. (cons Gy nil) ..))) ..))))
-      (OfeMor (rev_curry (tcurry (fun x1 => .. (tcurry (fun xn (_ : tuple_type tnil) => nil)) ..))))
-      (OfeMor (rev_curry (tcurry (fun x1 => .. (tcurry (fun xn (_ : tuple_type tnil) x => S2)) ..))))
-      (OfeMor (rev_curry (tcurry (fun x1 => .. (tcurry (fun xn (_ : tuple_type tnil) => E)) ..))))
-      (OfeMor (rev_curry (tcurry (fun x1 => .. (tcurry (fun xn (_ : tuple_type tnil) x _ => fold_right_sepcon (cons SQx%I .. (cons SQy%I nil) ..))) ..)))))
+      (OfeMor(ofe_mor_ne := _) (rev_curry (tcurry (fun x1 => .. (tcurry (fun xn (_ : tuple_type tnil) => nil)) ..))))
+      (OfeMor(ofe_mor_ne := _) (rev_curry (tcurry (fun x1 => .. (tcurry (fun xn (_ : tuple_type tnil) => nil)) ..))))
+      (OfeMor(ofe_mor_ne := _) (rev_curry (tcurry (fun x1 => .. (tcurry (fun xn (_ : tuple_type tnil) => (cons Gx .. (cons Gy nil) ..))) ..))))
+      (OfeMor(ofe_mor_ne := _) (rev_curry (tcurry (fun x1 => .. (tcurry (fun xn (_ : tuple_type tnil) => nil)) ..))))
+      (OfeMor(ofe_mor_ne := _) (rev_curry (tcurry (fun x1 => .. (tcurry (fun xn (_ : tuple_type tnil) x => S2)) ..))))
+      (OfeMor(ofe_mor_ne := _) (rev_curry (tcurry (fun x1 => .. (tcurry (fun xn (_ : tuple_type tnil) => E)) ..))))
+      (OfeMor(ofe_mor_ne := _) (rev_curry (tcurry (fun x1 => .. (tcurry (fun xn (_ : tuple_type tnil) x _ => fold_right_sepcon (cons SQx%I .. (cons SQy%I nil) ..))) ..)))))
   (atomic_spec_post0 W
-      (OfeMor (rev_curry (tcurry (fun x1 => .. (tcurry (fun xn (_ : tuple_type tnil) => (cons LQx%assert3 .. (cons LQy%assert3 nil) ..))) ..))))
-      (OfeMor (rev_curry (tcurry (fun x1 => .. (tcurry (fun xn (_ : tuple_type tnil) => nil)) ..))))))
+      (OfeMor(ofe_mor_ne := _) (rev_curry (tcurry (fun x1 => .. (tcurry (fun xn (_ : tuple_type tnil) => (cons LQx%assert3 .. (cons LQy%assert3 nil) ..))) ..))))
+      (OfeMor(ofe_mor_ne := _)(B := list mpred) (rev_curry (tcurry (fun x1 => .. (tcurry (fun xn (_ : tuple_type tnil) => nil)) ..))))))
   (at level 200, x1 closed binder, xn closed binder, x at level 0, E at level 0, S2 at level 0).
 
 Notation "'ATOMIC' 'TYPE' W 'OBJ' x 'INVS' E 'WITH' x1 , .. , xn 'PRE'  [ ] 'PROP' () 'PARAMS' () 'GLOBALS' ( Gx ; .. ; Gy ) 'SEP' () '|' S2 'POST' [ tz ] 'PROP' () 'LOCAL' () 'SEP' () '|' ( SQx ; .. ; SQy )" :=
   (mk_funspec (pair nil tz) cc_default ⊤ (atomic_spec_type0 W)
    (atomic_spec_pre0 W
-      (OfeMor (rev_curry (tcurry (fun x1 => .. (tcurry (fun xn (_ : tuple_type tnil) => nil)) ..))))
-      (OfeMor (rev_curry (tcurry (fun x1 => .. (tcurry (fun xn (_ : tuple_type tnil) => nil)) ..))))
-      (OfeMor (rev_curry (tcurry (fun x1 => .. (tcurry (fun xn (_ : tuple_type tnil) => (cons Gx .. (cons Gy nil) ..))) ..))))
-      (OfeMor (rev_curry (tcurry (fun x1 => .. (tcurry (fun xn (_ : tuple_type tnil) => nil)) ..))))
-      (OfeMor (rev_curry (tcurry (fun x1 => .. (tcurry (fun xn (_ : tuple_type tnil) x => S2)) ..))))
-      (OfeMor (rev_curry (tcurry (fun x1 => .. (tcurry (fun xn (_ : tuple_type tnil) => E)) ..))))
-      (OfeMor (rev_curry (tcurry (fun x1 => .. (tcurry (fun xn (_ : tuple_type tnil) x _ => fold_right_sepcon (cons SQx%I .. (cons SQy%I nil) ..))) ..)))))
+      (OfeMor(ofe_mor_ne := _) (rev_curry (tcurry (fun x1 => .. (tcurry (fun xn (_ : tuple_type tnil) => nil)) ..))))
+      (OfeMor(ofe_mor_ne := _) (rev_curry (tcurry (fun x1 => .. (tcurry (fun xn (_ : tuple_type tnil) => nil)) ..))))
+      (OfeMor(ofe_mor_ne := _) (rev_curry (tcurry (fun x1 => .. (tcurry (fun xn (_ : tuple_type tnil) => (cons Gx .. (cons Gy nil) ..))) ..))))
+      (OfeMor(ofe_mor_ne := _)(B := list mpred) (rev_curry (tcurry (fun x1 => .. (tcurry (fun xn (_ : tuple_type tnil) => nil)) ..))))
+      (OfeMor(ofe_mor_ne := _) (rev_curry (tcurry (fun x1 => .. (tcurry (fun xn (_ : tuple_type tnil) x => S2)) ..))))
+      (OfeMor(ofe_mor_ne := _) (rev_curry (tcurry (fun x1 => .. (tcurry (fun xn (_ : tuple_type tnil) => E)) ..))))
+      (OfeMor(ofe_mor_ne := _) (rev_curry (tcurry (fun x1 => .. (tcurry (fun xn (_ : tuple_type tnil) x _ => fold_right_sepcon (cons SQx%I .. (cons SQy%I nil) ..))) ..)))))
   (atomic_spec_post0 W
-      (OfeMor (rev_curry (tcurry (fun x1 => .. (tcurry (fun xn (_ : tuple_type tnil) => nil)) ..))))
-      (OfeMor (rev_curry (tcurry (fun x1 => .. (tcurry (fun xn (_ : tuple_type tnil) => nil)) ..))))))
+      (OfeMor(ofe_mor_ne := _)(B := leibnizO (list localdef)) (rev_curry (tcurry (fun x1 => .. (tcurry (fun xn (_ : tuple_type tnil) => nil)) ..))))
+      (OfeMor(ofe_mor_ne := _)(B := list mpred) (rev_curry (tcurry (fun x1 => .. (tcurry (fun xn (_ : tuple_type tnil) => nil)) ..))))))
   (at level 200, x1 closed binder, xn closed binder, x at level 0, E at level 0, S2 at level 0).
 
 Notation "'ATOMIC' 'TYPE' W 'INVS' E 'WITH' x1 , .. , xn 'PRE'  [ u , .. , v ] 'PROP' () 'PARAMS' ( Lx ; .. ; Ly ) 'GLOBALS' ( Gx ; .. ; Gy ) 'SEP' ( S1x ; .. ; S1y ) '|' S2 'POST' [ tz ] 'PROP' () 'LOCAL' () 'SEP' ( SPx ; .. ; SPy ) '|' ( SQx ; .. ; SQy )" :=
   (mk_funspec (pair (cons u%type .. (cons v%type nil) ..) tz) cc_default ⊤ (atomic_spec_type0 W)
    (atomic_spec_pre0 W
-      (OfeMor (rev_curry (tcurry (fun x1 => .. (tcurry (fun xn (_ : tuple_type tnil) => nil)) ..))))
-      (OfeMor (rev_curry (tcurry (fun x1 => .. (tcurry (fun xn (_ : tuple_type tnil) => (cons Lx%type .. (cons Ly%type nil) ..))) ..))))
-      (OfeMor (rev_curry (tcurry (fun x1 => .. (tcurry (fun xn (_ : tuple_type tnil) => (cons Gx .. (cons Gy nil) ..))) ..))))
-      (OfeMor (rev_curry (tcurry (fun x1 => .. (tcurry (fun xn (_ : tuple_type tnil) => (cons S1x%I .. (cons S1y%I nil) ..))) ..))))
-      (OfeMor (rev_curry (tcurry (fun x1 => .. (tcurry (fun xn (_ : tuple_type tnil) (_:unit) => S2)) ..))))
-      (OfeMor (rev_curry (tcurry (fun x1 => .. (tcurry (fun xn (_ : tuple_type tnil) => E)) ..))))
-      (OfeMor (rev_curry (tcurry (fun x1 => .. (tcurry (fun xn (_ : tuple_type tnil) _ _ => fold_right_sepcon (cons SQx%I .. (cons SQy%I nil) ..))) ..)))))
+      (OfeMor(ofe_mor_ne := _) (rev_curry (tcurry (fun x1 => .. (tcurry (fun xn (_ : tuple_type tnil) => nil)) ..))))
+      (OfeMor(ofe_mor_ne := _) (rev_curry (tcurry (fun x1 => .. (tcurry (fun xn (_ : tuple_type tnil) => (cons Lx%type .. (cons Ly%type nil) ..))) ..))))
+      (OfeMor(ofe_mor_ne := _) (rev_curry (tcurry (fun x1 => .. (tcurry (fun xn (_ : tuple_type tnil) => (cons Gx .. (cons Gy nil) ..))) ..))))
+      (OfeMor(ofe_mor_ne := _) (rev_curry (tcurry (fun x1 => .. (tcurry (fun xn (_ : tuple_type tnil) => (cons S1x%I .. (cons S1y%I nil) ..))) ..))))
+      (OfeMor(ofe_mor_ne := _) (rev_curry (tcurry (fun x1 => .. (tcurry (fun xn (_ : tuple_type tnil) (_:unit) => S2)) ..))))
+      (OfeMor(ofe_mor_ne := _) (rev_curry (tcurry (fun x1 => .. (tcurry (fun xn (_ : tuple_type tnil) => E)) ..))))
+      (OfeMor(ofe_mor_ne := _) (rev_curry (tcurry (fun x1 => .. (tcurry (fun xn (_ : tuple_type tnil) _ _ => fold_right_sepcon (cons SQx%I .. (cons SQy%I nil) ..))) ..)))))
   (atomic_spec_post0 W
-      (OfeMor (rev_curry (tcurry (fun x1 => .. (tcurry (fun xn (_ : tuple_type tnil) => nil)) ..))))
-      (OfeMor (rev_curry (tcurry (fun x1 => .. (tcurry (fun xn (_ : tuple_type tnil) => (cons SPx%assert5%assert3 .. (cons SPy%assert5%assert3 nil) ..))) ..))))))
+      (OfeMor(ofe_mor_ne := _)(B := leibnizO (list localdef)) (rev_curry (tcurry (fun x1 => .. (tcurry (fun xn (_ : tuple_type tnil) => nil)) ..))))
+      (OfeMor(ofe_mor_ne := _) (rev_curry (tcurry (fun x1 => .. (tcurry (fun xn (_ : tuple_type tnil) => (cons SPx%assert5%assert3 .. (cons SPy%assert5%assert3 nil) ..))) ..))))))
   (at level 200, x1 closed binder, xn closed binder, E at level 0, S2 at level 0).
 
 Notation "'ATOMIC' 'TYPE' W 'OBJ' x 'INVS' E 'WITH' x1 , .. , xn 'PRE'  [ u , .. , v ] 'PROP' () 'PARAMS' ( Lx ; .. ; Ly ) 'GLOBALS' ( Gx ; .. ; Gy ) 'SEP' ( S1x ; .. ; S1y ) '|' S2 'POST' [ tz ] 'PROP' () 'LOCAL' () 'SEP' ( SPx ; .. ; SPy ) '|' ( SQx ; .. ; SQy )" :=
   (mk_funspec (pair (cons u%type .. (cons v%type nil) ..) tz) cc_default ⊤ (atomic_spec_type0 W)
    (atomic_spec_pre0 W
-      (OfeMor (rev_curry (tcurry (fun x1 => .. (tcurry (fun xn (_ : tuple_type tnil) => nil)) ..))))
-      (OfeMor (rev_curry (tcurry (fun x1 => .. (tcurry (fun xn (_ : tuple_type tnil) => (cons Lx%type .. (cons Ly%type nil) ..))) ..))))
-      (OfeMor (rev_curry (tcurry (fun x1 => .. (tcurry (fun xn (_ : tuple_type tnil) => (cons Gx .. (cons Gy nil) ..))) ..))))
-      (OfeMor (rev_curry (tcurry (fun x1 => .. (tcurry (fun xn (_ : tuple_type tnil) => (cons S1x%I .. (cons S1y%I nil) ..))) ..))))
-      (OfeMor (rev_curry (tcurry (fun x1 => .. (tcurry (fun xn (_ : tuple_type tnil) x => S2)) ..))))       (OfeMor (rev_curry (tcurry (fun x1 => .. (tcurry (fun xn (_ : tuple_type tnil) => E)) ..))))
-      (OfeMor (rev_curry (tcurry (fun x1 => .. (tcurry (fun xn (_ : tuple_type tnil) x _ => fold_right_sepcon (cons SQx%I .. (cons SQy%I nil) ..))) ..)))))
+      (OfeMor(ofe_mor_ne := _) (rev_curry (tcurry (fun x1 => .. (tcurry (fun xn (_ : tuple_type tnil) => nil)) ..))))
+      (OfeMor(ofe_mor_ne := _) (rev_curry (tcurry (fun x1 => .. (tcurry (fun xn (_ : tuple_type tnil) => (cons Lx%type .. (cons Ly%type nil) ..))) ..))))
+      (OfeMor(ofe_mor_ne := _) (rev_curry (tcurry (fun x1 => .. (tcurry (fun xn (_ : tuple_type tnil) => (cons Gx .. (cons Gy nil) ..))) ..))))
+      (OfeMor(ofe_mor_ne := _) (rev_curry (tcurry (fun x1 => .. (tcurry (fun xn (_ : tuple_type tnil) => (cons S1x%I .. (cons S1y%I nil) ..))) ..))))
+      (OfeMor(ofe_mor_ne := _) (rev_curry (tcurry (fun x1 => .. (tcurry (fun xn (_ : tuple_type tnil) x => S2)) ..))))       (OfeMor(ofe_mor_ne := _) (rev_curry (tcurry (fun x1 => .. (tcurry (fun xn (_ : tuple_type tnil) => E)) ..))))
+      (OfeMor(ofe_mor_ne := _) (rev_curry (tcurry (fun x1 => .. (tcurry (fun xn (_ : tuple_type tnil) x _ => fold_right_sepcon (cons SQx%I .. (cons SQy%I nil) ..))) ..)))))
   (atomic_spec_post0 W
-      (OfeMor (rev_curry (tcurry (fun x1 => .. (tcurry (fun xn (_ : tuple_type tnil) => nil)) ..))))
-      (OfeMor (rev_curry (tcurry (fun x1 => .. (tcurry (fun xn (_ : tuple_type tnil) => (cons SPx%assert5%assert3 .. (cons SPy%assert5%assert3 nil) ..))) ..))))))
+      (OfeMor(ofe_mor_ne := _)(B := leibnizO (list localdef)) (rev_curry (tcurry (fun x1 => .. (tcurry (fun xn (_ : tuple_type tnil) => nil)) ..))))
+      (OfeMor(ofe_mor_ne := _) (rev_curry (tcurry (fun x1 => .. (tcurry (fun xn (_ : tuple_type tnil) => (cons SPx%assert5%assert3 .. (cons SPy%assert5%assert3 nil) ..))) ..))))))
   (at level 200, x1 closed binder, xn closed binder, x at level 0, E at level 0, S2 at level 0).
 
 Notation "'ATOMIC' 'TYPE' W 'INVS' E 'WITH' x1 , .. , xn 'PRE'  [ u , .. , v ] 'PROP' () 'PARAMS' ( Lx ; .. ; Ly ) 'SEP' () '|' S2 'POST' [ tz ] 'PROP' () 'LOCAL' () 'SEP' () '|' ( SQx ; .. ; SQy )" :=
   (mk_funspec (pair (cons u%type .. (cons v%type nil) ..) tz) cc_default ⊤ (atomic_spec_type0 W)
    (atomic_spec_pre0 W
-      (OfeMor (rev_curry (tcurry (fun x1 => .. (tcurry (fun xn (_ : tuple_type tnil) => nil)) ..))))
-      (OfeMor (rev_curry (tcurry (fun x1 => .. (tcurry (fun xn (_ : tuple_type tnil) => (cons Lx%type .. (cons Ly%type nil) ..))) ..))))
-      (OfeMor (rev_curry (tcurry (fun x1 => .. (tcurry (fun xn (_ : tuple_type tnil) => nil)) ..))))
-      (OfeMor (rev_curry (tcurry (fun x1 => .. (tcurry (fun xn (_ : tuple_type tnil) => nil)) ..))))
-      (OfeMor (rev_curry (tcurry (fun x1 => .. (tcurry (fun xn (_ : tuple_type tnil) (_:unit) => S2)) ..))))
-      (OfeMor (rev_curry (tcurry (fun x1 => .. (tcurry (fun xn (_ : tuple_type tnil) => E)) ..))))
-      (OfeMor (rev_curry (tcurry (fun x1 => .. (tcurry (fun xn (_ : tuple_type tnil) _ _ => fold_right_sepcon (cons SQx%I .. (cons SQy%I nil) ..))) ..)))))
+      (OfeMor(ofe_mor_ne := _) (rev_curry (tcurry (fun x1 => .. (tcurry (fun xn (_ : tuple_type tnil) => nil)) ..))))
+      (OfeMor(ofe_mor_ne := _) (rev_curry (tcurry (fun x1 => .. (tcurry (fun xn (_ : tuple_type tnil) => (cons Lx%type .. (cons Ly%type nil) ..))) ..))))
+      (OfeMor(ofe_mor_ne := _)(B := leibnizO (list globals)) (rev_curry (tcurry (fun x1 => .. (tcurry (fun xn (_ : tuple_type tnil) => nil)) ..))))
+      (OfeMor(ofe_mor_ne := _)(B := list mpred) (rev_curry (tcurry (fun x1 => .. (tcurry (fun xn (_ : tuple_type tnil) => nil)) ..))))
+      (OfeMor(ofe_mor_ne := _) (rev_curry (tcurry (fun x1 => .. (tcurry (fun xn (_ : tuple_type tnil) (_:unit) => S2)) ..))))
+      (OfeMor(ofe_mor_ne := _) (rev_curry (tcurry (fun x1 => .. (tcurry (fun xn (_ : tuple_type tnil) => E)) ..))))
+      (OfeMor(ofe_mor_ne := _) (rev_curry (tcurry (fun x1 => .. (tcurry (fun xn (_ : tuple_type tnil) _ _ => fold_right_sepcon (cons SQx%I .. (cons SQy%I nil) ..))) ..)))))
   (atomic_spec_post0 W
-      (OfeMor (rev_curry (tcurry (fun x1 => .. (tcurry (fun xn (_ : tuple_type tnil) => nil)) ..))))
-      (OfeMor (rev_curry (tcurry (fun x1 => .. (tcurry (fun xn (_ : tuple_type tnil) => nil)) ..))))))
+      (OfeMor(ofe_mor_ne := _)(B := leibnizO (list localdef)) (rev_curry (tcurry (fun x1 => .. (tcurry (fun xn (_ : tuple_type tnil) => nil)) ..))))
+      (OfeMor(ofe_mor_ne := _)(B := list mpred) (rev_curry (tcurry (fun x1 => .. (tcurry (fun xn (_ : tuple_type tnil) => nil)) ..))))))
   (at level 200, x1 closed binder, xn closed binder, E at level 0, S2 at level 0).
 
 Notation "'ATOMIC' 'TYPE' W 'OBJ' x 'INVS' E 'WITH' x1 , .. , xn 'PRE'  [ u , .. , v ] 'PROP' () 'PARAMS' ( Lx ; .. ; Ly ) 'SEP' () '|' S2 'POST' [ tz ] 'PROP' () 'LOCAL' () 'SEP' () '|' ( SQx ; .. ; SQy )" :=
   (mk_funspec (pair (cons u%type .. (cons v%type nil) ..) tz) cc_default ⊤ (atomic_spec_type0 W)
    (atomic_spec_pre0 W
-      (OfeMor (rev_curry (tcurry (fun x1 => .. (tcurry (fun xn (_ : tuple_type tnil) => nil)) ..))))
-      (OfeMor (rev_curry (tcurry (fun x1 => .. (tcurry (fun xn (_ : tuple_type tnil) => (cons Lx%type .. (cons Ly%type nil) ..))) ..))))
-      (OfeMor (rev_curry (tcurry (fun x1 => .. (tcurry (fun xn (_ : tuple_type tnil) => nil)) ..))))
-      (OfeMor (rev_curry (tcurry (fun x1 => .. (tcurry (fun xn (_ : tuple_type tnil) => nil)) ..))))
-      (OfeMor (rev_curry (tcurry (fun x1 => .. (tcurry (fun xn (_ : tuple_type tnil) x => S2)) ..))))
-      (OfeMor (rev_curry (tcurry (fun x1 => .. (tcurry (fun xn (_ : tuple_type tnil) => E)) ..))))
-      (OfeMor (rev_curry (tcurry (fun x1 => .. (tcurry (fun xn (_ : tuple_type tnil) x _ => fold_right_sepcon (cons SQx%I .. (cons SQy%I nil) ..))) ..)))))
+      (OfeMor(ofe_mor_ne := _) (rev_curry (tcurry (fun x1 => .. (tcurry (fun xn (_ : tuple_type tnil) => nil)) ..))))
+      (OfeMor(ofe_mor_ne := _) (rev_curry (tcurry (fun x1 => .. (tcurry (fun xn (_ : tuple_type tnil) => (cons Lx%type .. (cons Ly%type nil) ..))) ..))))
+      (OfeMor(ofe_mor_ne := _)(B := leibnizO (list globals)) (rev_curry (tcurry (fun x1 => .. (tcurry (fun xn (_ : tuple_type tnil) => nil)) ..))))
+      (OfeMor(ofe_mor_ne := _)(B := list mpred) (rev_curry (tcurry (fun x1 => .. (tcurry (fun xn (_ : tuple_type tnil) => nil)) ..))))
+      (OfeMor(ofe_mor_ne := _) (rev_curry (tcurry (fun x1 => .. (tcurry (fun xn (_ : tuple_type tnil) x => S2)) ..))))
+      (OfeMor(ofe_mor_ne := _) (rev_curry (tcurry (fun x1 => .. (tcurry (fun xn (_ : tuple_type tnil) => E)) ..))))
+      (OfeMor(ofe_mor_ne := _) (rev_curry (tcurry (fun x1 => .. (tcurry (fun xn (_ : tuple_type tnil) x _ => fold_right_sepcon (cons SQx%I .. (cons SQy%I nil) ..))) ..)))))
   (atomic_spec_post0 W
-      (OfeMor (rev_curry (tcurry (fun x1 => .. (tcurry (fun xn (_ : tuple_type tnil) => nil)) ..))))
-      (OfeMor (rev_curry (tcurry (fun x1 => .. (tcurry (fun xn (_ : tuple_type tnil) => nil)) ..))))))
+      (OfeMor(ofe_mor_ne := _)(B := leibnizO (list localdef)) (rev_curry (tcurry (fun x1 => .. (tcurry (fun xn (_ : tuple_type tnil) => nil)) ..))))
+      (OfeMor(ofe_mor_ne := _)(B := list mpred) (rev_curry (tcurry (fun x1 => .. (tcurry (fun xn (_ : tuple_type tnil) => nil)) ..))))))
   (at level 200, x1 closed binder, xn closed binder, x at level 0, E at level 0, S2 at level 0).
 
 Notation "'ATOMIC' 'TYPE' W 'OBJ' x 'INVS' E 'WITH' x1 , .. , xn 'PRE'  [ u , .. , v ] 'PROP' () 'PARAMS' ( Lx ; .. ; Ly ) 'SEP' ( S1x ; .. ; S1y ) '|' S2 'POST' [ tz ] 'PROP' () 'LOCAL' () 'SEP' () '|' ( SQx ; .. ; SQy )" :=
   (mk_funspec (pair (cons u%type .. (cons v%type nil) ..) tz) cc_default ⊤ (atomic_spec_type0 W)
    (atomic_spec_pre0 W
-      (OfeMor (rev_curry (tcurry (fun x1 => .. (tcurry (fun xn (_ : tuple_type tnil) => nil)) ..))))
-      (OfeMor (rev_curry (tcurry (fun x1 => .. (tcurry (fun xn (_ : tuple_type tnil) => (cons Lx%type .. (cons Ly%type nil) ..))) ..))))
-      (OfeMor (rev_curry (tcurry (fun x1 => .. (tcurry (fun xn (_ : tuple_type tnil) => nil)) ..))))
-      (OfeMor (rev_curry (tcurry (fun x1 => .. (tcurry (fun xn (_ : tuple_type tnil) => (cons S1x%I .. (cons S1y%I nil) ..))) ..))))
-      (OfeMor (rev_curry (tcurry (fun x1 => .. (tcurry (fun xn (_ : tuple_type tnil) x => S2)) ..))))
-      (OfeMor (rev_curry (tcurry (fun x1 => .. (tcurry (fun xn (_ : tuple_type tnil) => E)) ..))))
-      (OfeMor (rev_curry (tcurry (fun x1 => .. (tcurry (fun xn (_ : tuple_type tnil) x _ => fold_right_sepcon (cons SQx%I .. (cons SQy%I nil) ..))) ..)))))
+      (OfeMor(ofe_mor_ne := _) (rev_curry (tcurry (fun x1 => .. (tcurry (fun xn (_ : tuple_type tnil) => nil)) ..))))
+      (OfeMor(ofe_mor_ne := _) (rev_curry (tcurry (fun x1 => .. (tcurry (fun xn (_ : tuple_type tnil) => (cons Lx%type .. (cons Ly%type nil) ..))) ..))))
+      (OfeMor(ofe_mor_ne := _)(B := leibnizO (list globals)) (rev_curry (tcurry (fun x1 => .. (tcurry (fun xn (_ : tuple_type tnil) => nil)) ..))))
+      (OfeMor(ofe_mor_ne := _) (rev_curry (tcurry (fun x1 => .. (tcurry (fun xn (_ : tuple_type tnil) => (cons S1x%I .. (cons S1y%I nil) ..))) ..))))
+      (OfeMor(ofe_mor_ne := _) (rev_curry (tcurry (fun x1 => .. (tcurry (fun xn (_ : tuple_type tnil) x => S2)) ..))))
+      (OfeMor(ofe_mor_ne := _) (rev_curry (tcurry (fun x1 => .. (tcurry (fun xn (_ : tuple_type tnil) => E)) ..))))
+      (OfeMor(ofe_mor_ne := _) (rev_curry (tcurry (fun x1 => .. (tcurry (fun xn (_ : tuple_type tnil) x _ => fold_right_sepcon (cons SQx%I .. (cons SQy%I nil) ..))) ..)))))
   (atomic_spec_post0 W
-      (OfeMor (rev_curry (tcurry (fun x1 => .. (tcurry (fun xn (_ : tuple_type tnil) => nil)) ..))))
-      (OfeMor (rev_curry (tcurry (fun x1 => .. (tcurry (fun xn (_ : tuple_type tnil) => nil)) ..))))))
+      (OfeMor(ofe_mor_ne := _)(B := leibnizO (list localdef)) (rev_curry (tcurry (fun x1 => .. (tcurry (fun xn (_ : tuple_type tnil) => nil)) ..))))
+      (OfeMor(ofe_mor_ne := _)(B := list mpred) (rev_curry (tcurry (fun x1 => .. (tcurry (fun xn (_ : tuple_type tnil) => nil)) ..))))))
   (at level 200, x1 closed binder, xn closed binder, x at level 0, E at level 0, S2 at level 0).
 
 Notation "'ATOMIC' 'TYPE' W 'OBJ' x 'INVS' E 'WITH' x1 , .. , xn 'PRE'  [ u , .. , v ] 'PROP' () 'PARAMS' ( Lx ; .. ; Ly ) 'SEP' ( S1x ; .. ; S1y ) '|' S2 'POST' [ tz ] 'PROP' () 'LOCAL' () 'SEP' ( SPx ; .. ; SPy ) '|' ( SQx ; .. ; SQy )" :=
   (mk_funspec (pair (cons u%type .. (cons v%type nil) ..) tz) cc_default ⊤ (atomic_spec_type0 W)
    (atomic_spec_pre0 W
-      (OfeMor (rev_curry (tcurry (fun x1 => .. (tcurry (fun xn (_ : tuple_type tnil) => nil)) ..))))
-      (OfeMor (rev_curry (tcurry (fun x1 => .. (tcurry (fun xn (_ : tuple_type tnil) => (cons Lx%type .. (cons Ly%type nil) ..))) ..))))
-      (OfeMor (rev_curry (tcurry (fun x1 => .. (tcurry (fun xn (_ : tuple_type tnil) => nil)) ..))))
-      (OfeMor (rev_curry (tcurry (fun x1 => .. (tcurry (fun xn (_ : tuple_type tnil) => (cons S1x%I .. (cons S1y%I nil) ..))) ..))))
-      (OfeMor (rev_curry (tcurry (fun x1 => .. (tcurry (fun xn (_ : tuple_type tnil) x => S2)) ..))))
-      (OfeMor (rev_curry (tcurry (fun x1 => .. (tcurry (fun xn (_ : tuple_type tnil) => E)) ..))))
-      (OfeMor (rev_curry (tcurry (fun x1 => .. (tcurry (fun xn (_ : tuple_type tnil) x _ => fold_right_sepcon (cons SQx%I .. (cons SQy%I nil) ..))) ..)))))
+      (OfeMor(ofe_mor_ne := _) (rev_curry (tcurry (fun x1 => .. (tcurry (fun xn (_ : tuple_type tnil) => nil)) ..))))
+      (OfeMor(ofe_mor_ne := _) (rev_curry (tcurry (fun x1 => .. (tcurry (fun xn (_ : tuple_type tnil) => (cons Lx%type .. (cons Ly%type nil) ..))) ..))))
+      (OfeMor(ofe_mor_ne := _)(B := leibnizO (list globals)) (rev_curry (tcurry (fun x1 => .. (tcurry (fun xn (_ : tuple_type tnil) => nil)) ..))))
+      (OfeMor(ofe_mor_ne := _) (rev_curry (tcurry (fun x1 => .. (tcurry (fun xn (_ : tuple_type tnil) => (cons S1x%I .. (cons S1y%I nil) ..))) ..))))
+      (OfeMor(ofe_mor_ne := _) (rev_curry (tcurry (fun x1 => .. (tcurry (fun xn (_ : tuple_type tnil) x => S2)) ..))))
+      (OfeMor(ofe_mor_ne := _) (rev_curry (tcurry (fun x1 => .. (tcurry (fun xn (_ : tuple_type tnil) => E)) ..))))
+      (OfeMor(ofe_mor_ne := _) (rev_curry (tcurry (fun x1 => .. (tcurry (fun xn (_ : tuple_type tnil) x _ => fold_right_sepcon (cons SQx%I .. (cons SQy%I nil) ..))) ..)))))
   (atomic_spec_post0 W
-      (OfeMor (rev_curry (tcurry (fun x1 => .. (tcurry (fun xn (_ : tuple_type tnil) => nil)) ..))))
-      (OfeMor (rev_curry (tcurry (fun x1 => .. (tcurry (fun xn (_ : tuple_type tnil) => cons SPx%assert5%assert3 .. (cons SPy%assert5%assert3 nil) ..)) ..))))))
+      (OfeMor(ofe_mor_ne := _)(B := leibnizO (list localdef)) (rev_curry (tcurry (fun x1 => .. (tcurry (fun xn (_ : tuple_type tnil) => nil)) ..))))
+      (OfeMor(ofe_mor_ne := _) (rev_curry (tcurry (fun x1 => .. (tcurry (fun xn (_ : tuple_type tnil) => cons SPx%assert5%assert3 .. (cons SPy%assert5%assert3 nil) ..)) ..))))))
   (at level 200, x1 closed binder, xn closed binder, x at level 0, E at level 0, S2 at level 0).
 
 Notation "'ATOMIC' 'TYPE' W 'INVS' E 'WITH' x1 , .. , xn 'PRE'  [ u , .. , v ] 'PROP' () 'PARAMS' ( Lx ; .. ; Ly ) 'SEP' ( S1x ; .. ; S1y ) '|' S2 'POST' [ tz ] 'PROP' () 'LOCAL' () 'SEP' ( SPx ; .. ; SPy ) '|' ( SQx ; .. ; SQy )" :=
   (mk_funspec (pair (cons u%type .. (cons v%type nil) ..) tz) cc_default ⊤ (atomic_spec_type0 W)
    (atomic_spec_pre0 W
-      (OfeMor (rev_curry (tcurry (fun x1 => .. (tcurry (fun xn (_ : tuple_type tnil) => nil)) ..))))
-      (OfeMor (rev_curry (tcurry (fun x1 => .. (tcurry (fun xn (_ : tuple_type tnil) => (cons Lx%type .. (cons Ly%type nil) ..))) ..))))
-      (OfeMor (rev_curry (tcurry (fun x1 => .. (tcurry (fun xn (_ : tuple_type tnil) => nil)) ..))))
-      (OfeMor (rev_curry (tcurry (fun x1 => .. (tcurry (fun xn (_ : tuple_type tnil) => (cons S1x%I .. (cons S1y%I nil) ..))) ..))))
-      (OfeMor (rev_curry (tcurry (fun x1 => .. (tcurry (fun xn (_ : tuple_type tnil) (_ : unit) => S2)) ..))))
-      (OfeMor (rev_curry (tcurry (fun x1 => .. (tcurry (fun xn (_ : tuple_type tnil) => E)) ..))))
-      (OfeMor (rev_curry (tcurry (fun x1 => .. (tcurry (fun xn (_ : tuple_type tnil) (_ : unit) _ => fold_right_sepcon (cons SQx%I .. (cons SQy%I nil) ..))) ..)))))
+      (OfeMor(ofe_mor_ne := _) (rev_curry (tcurry (fun x1 => .. (tcurry (fun xn (_ : tuple_type tnil) => nil)) ..))))
+      (OfeMor(ofe_mor_ne := _) (rev_curry (tcurry (fun x1 => .. (tcurry (fun xn (_ : tuple_type tnil) => (cons Lx%type .. (cons Ly%type nil) ..))) ..))))
+      (OfeMor(ofe_mor_ne := _)(B := leibnizO (list globals)) (rev_curry (tcurry (fun x1 => .. (tcurry (fun xn (_ : tuple_type tnil) => nil)) ..))))
+      (OfeMor(ofe_mor_ne := _) (rev_curry (tcurry (fun x1 => .. (tcurry (fun xn (_ : tuple_type tnil) => (cons S1x%I .. (cons S1y%I nil) ..))) ..))))
+      (OfeMor(ofe_mor_ne := _) (rev_curry (tcurry (fun x1 => .. (tcurry (fun xn (_ : tuple_type tnil) (_ : unit) => S2)) ..))))
+      (OfeMor(ofe_mor_ne := _) (rev_curry (tcurry (fun x1 => .. (tcurry (fun xn (_ : tuple_type tnil) => E)) ..))))
+      (OfeMor(ofe_mor_ne := _) (rev_curry (tcurry (fun x1 => .. (tcurry (fun xn (_ : tuple_type tnil) (_ : unit) _ => fold_right_sepcon (cons SQx%I .. (cons SQy%I nil) ..))) ..)))))
   (atomic_spec_post0 W
-      (OfeMor (rev_curry (tcurry (fun x1 => .. (tcurry (fun xn (_ : tuple_type tnil) => nil)) ..))))
-      (OfeMor (rev_curry (tcurry (fun x1 => .. (tcurry (fun xn (_ : tuple_type tnil) => cons SPx%assert5%assert3 .. (cons SPy%assert5%assert3 nil) ..)) ..))))))
+      (OfeMor(ofe_mor_ne := _)(B := leibnizO (list localdef)) (rev_curry (tcurry (fun x1 => .. (tcurry (fun xn (_ : tuple_type tnil) => nil)) ..))))
+      (OfeMor(ofe_mor_ne := _) (rev_curry (tcurry (fun x1 => .. (tcurry (fun xn (_ : tuple_type tnil) => cons SPx%assert5%assert3 .. (cons SPy%assert5%assert3 nil) ..)) ..))))))
   (at level 200, x1 closed binder, xn closed binder, E at level 0, S2 at level 0).
 
 Notation "'ATOMIC' 'TYPE' W 'INVS' E 'WITH' x1 , .. , xn 'PRE'  [ u , .. , v ] 'PROP' ( Px ; .. ; Py ) 'PARAMS' ( Lx ; .. ; Ly ) 'SEP' ( S1x ; .. ; S1y ) '|' S2 'POST' [ tz ] 'PROP' () 'LOCAL' () 'SEP' ( SPx ; .. ; SPy ) '|' ( SQx ; .. ; SQy )" :=
   (mk_funspec (pair (cons u%type .. (cons v%type nil) ..) tz) cc_default ⊤ (atomic_spec_type0 W)
    (atomic_spec_pre0 W
-      (rev_curry (tcurry (fun x1 => .. (tcurry (fun xn (_ : tuple_type tnil) => cons Px%type .. (cons Py%type nil) ..)) ..)))
-      (OfeMor (rev_curry (tcurry (fun x1 => .. (tcurry (fun xn (_ : tuple_type tnil) => (cons Lx%type .. (cons Ly%type nil) ..))) ..))))
-      (OfeMor (rev_curry (tcurry (fun x1 => .. (tcurry (fun xn (_ : tuple_type tnil) => nil)) ..))))
-      (OfeMor (rev_curry (tcurry (fun x1 => .. (tcurry (fun xn (_ : tuple_type tnil) => (cons S1x%I .. (cons S1y%I nil) ..))) ..))))
-      (OfeMor (rev_curry (tcurry (fun x1 => .. (tcurry (fun xn (_ : tuple_type tnil) (_ : unit) => S2)) ..))))
-      (OfeMor (rev_curry (tcurry (fun x1 => .. (tcurry (fun xn (_ : tuple_type tnil) => E)) ..))))
-      (OfeMor (rev_curry (tcurry (fun x1 => .. (tcurry (fun xn (_ : tuple_type tnil) (_ : unit) _ => fold_right_sepcon (cons SQx%I .. (cons SQy%I nil) ..))) ..)))))
+      (OfeMor(ofe_mor_ne := _) (rev_curry (tcurry (fun x1 => .. (tcurry (fun xn (_ : tuple_type tnil) => cons Px%type .. (cons Py%type nil) ..)) ..))))
+      (OfeMor(ofe_mor_ne := _) (rev_curry (tcurry (fun x1 => .. (tcurry (fun xn (_ : tuple_type tnil) => (cons Lx%type .. (cons Ly%type nil) ..))) ..))))
+      (OfeMor(ofe_mor_ne := _)(B := leibnizO (list globals)) (rev_curry (tcurry (fun x1 => .. (tcurry (fun xn (_ : tuple_type tnil) => nil)) ..))))
+      (OfeMor(ofe_mor_ne := _) (rev_curry (tcurry (fun x1 => .. (tcurry (fun xn (_ : tuple_type tnil) => (cons S1x%I .. (cons S1y%I nil) ..))) ..))))
+      (OfeMor(ofe_mor_ne := _) (rev_curry (tcurry (fun x1 => .. (tcurry (fun xn (_ : tuple_type tnil) (_ : unit) => S2)) ..))))
+      (OfeMor(ofe_mor_ne := _) (rev_curry (tcurry (fun x1 => .. (tcurry (fun xn (_ : tuple_type tnil) => E)) ..))))
+      (OfeMor(ofe_mor_ne := _) (rev_curry (tcurry (fun x1 => .. (tcurry (fun xn (_ : tuple_type tnil) (_ : unit) _ => fold_right_sepcon (cons SQx%I .. (cons SQy%I nil) ..))) ..)))))
   (atomic_spec_post0 W
-      (OfeMor (rev_curry (tcurry (fun x1 => .. (tcurry (fun xn (_ : tuple_type tnil) => nil)) ..))))
-      (OfeMor (rev_curry (tcurry (fun x1 => .. (tcurry (fun xn (_ : tuple_type tnil) => cons SPx%assert5%assert3 .. (cons SPy%assert5%assert3 nil) ..)) ..))))))
+      (OfeMor(ofe_mor_ne := _)(B := leibnizO (list localdef)) (rev_curry (tcurry (fun x1 => .. (tcurry (fun xn (_ : tuple_type tnil) => nil)) ..))))
+      (OfeMor(ofe_mor_ne := _) (rev_curry (tcurry (fun x1 => .. (tcurry (fun xn (_ : tuple_type tnil) => cons SPx%assert5%assert3 .. (cons SPy%assert5%assert3 nil) ..)) ..))))))
   (at level 200, x1 closed binder, xn closed binder, E at level 0, S2 at level 0).
 
 Notation "'ATOMIC' 'TYPE' W 'OBJ' x 'INVS' E 'WITH' x1 , .. , xn 'PRE'  [ u , .. , v ] 'PROP' ( Px ; .. ; Py ) 'PARAMS' ( Lx ; .. ; Ly ) 'SEP' ( S1x ; .. ; S1y ) '|' S2 'POST' [ tz ] 'PROP' () 'LOCAL' () 'SEP' ( SPx ; .. ; SPy ) '|' ( SQx ; .. ; SQy )" :=
   (mk_funspec (pair (cons u%type .. (cons v%type nil) ..) tz) cc_default ⊤ (atomic_spec_type0 W)
    (atomic_spec_pre0 W
-      (OfeMor (rev_curry (tcurry (fun x1 => .. (tcurry (fun xn (_ : tuple_type tnil) => (cons Px%type .. (cons Py%type nil) ..))) ..))))
-      (OfeMor (rev_curry (tcurry (fun x1 => .. (tcurry (fun xn (_ : tuple_type tnil) => (cons Lx%type .. (cons Ly%type nil) ..))) ..))))
-      (OfeMor (rev_curry (tcurry (fun x1 => .. (tcurry (fun xn (_ : tuple_type tnil) => nil)) ..))))
-      (OfeMor (rev_curry (tcurry (fun x1 => .. (tcurry (fun xn (_ : tuple_type tnil) => (cons S1x%I .. (cons S1y%I nil) ..))) ..))))
-      (OfeMor (rev_curry (tcurry (fun x1 => .. (tcurry (fun xn (_ : tuple_type tnil) x => S2)) ..))))
-      (OfeMor (rev_curry (tcurry (fun x1 => .. (tcurry (fun xn (_ : tuple_type tnil) => E)) ..))))
-      (OfeMor (rev_curry (tcurry (fun x1 => .. (tcurry (fun xn (_ : tuple_type tnil) x _ => fold_right_sepcon (cons SQx%I .. (cons SQy%I nil) ..))) ..)))))
+      (OfeMor(ofe_mor_ne := _) (rev_curry (tcurry (fun x1 => .. (tcurry (fun xn (_ : tuple_type tnil) => (cons Px%type .. (cons Py%type nil) ..))) ..))))
+      (OfeMor(ofe_mor_ne := _) (rev_curry (tcurry (fun x1 => .. (tcurry (fun xn (_ : tuple_type tnil) => (cons Lx%type .. (cons Ly%type nil) ..))) ..))))
+      (OfeMor(ofe_mor_ne := _)(B := leibnizO (list globals)) (rev_curry (tcurry (fun x1 => .. (tcurry (fun xn (_ : tuple_type tnil) => nil)) ..))))
+      (OfeMor(ofe_mor_ne := _) (rev_curry (tcurry (fun x1 => .. (tcurry (fun xn (_ : tuple_type tnil) => (cons S1x%I .. (cons S1y%I nil) ..))) ..))))
+      (OfeMor(ofe_mor_ne := _) (rev_curry (tcurry (fun x1 => .. (tcurry (fun xn (_ : tuple_type tnil) x => S2)) ..))))
+      (OfeMor(ofe_mor_ne := _) (rev_curry (tcurry (fun x1 => .. (tcurry (fun xn (_ : tuple_type tnil) => E)) ..))))
+      (OfeMor(ofe_mor_ne := _) (rev_curry (tcurry (fun x1 => .. (tcurry (fun xn (_ : tuple_type tnil) x _ => fold_right_sepcon (cons SQx%I .. (cons SQy%I nil) ..))) ..)))))
   (atomic_spec_post0 W
-      (OfeMor (rev_curry (tcurry (fun x1 => .. (tcurry (fun xn (_ : tuple_type tnil) => nil)) ..))))
-      (OfeMor (rev_curry (tcurry (fun x1 => .. (tcurry (fun xn (_ : tuple_type tnil) => cons SPx%assert5%assert3 .. (cons SPy%assert5%assert3 nil) ..)) ..))))))
+      (OfeMor(ofe_mor_ne := _)(B := leibnizO (list localdef)) (rev_curry (tcurry (fun x1 => .. (tcurry (fun xn (_ : tuple_type tnil) => nil)) ..))))
+      (OfeMor(ofe_mor_ne := _) (rev_curry (tcurry (fun x1 => .. (tcurry (fun xn (_ : tuple_type tnil) => cons SPx%assert5%assert3 .. (cons SPy%assert5%assert3 nil) ..)) ..))))))
   (at level 200, x1 closed binder, xn closed binder, x at level 0, E at level 0, S2 at level 0).
 
-(*Ltac atomic_nonexpansive_tac := try (let x := fresh "x" in intros ???? x;
-  repeat destruct x as [x ?]; unfold rev_curry, tcurry; simpl; auto); try solve_proper.*)
+Ltac atomic_nonexpansive_tac := try (let x := fresh "x" in let y := fresh "y" in let H := fresh "Hdist" in intros ? x y H;
+  repeat (destruct x as [x ?]; try destruct y as [y ?]; try destruct H as [H ?];
+    try (hnf in H; simpl in H; match type of H with _ = ?b => subst b end)); unfold rev_curry, tcurry; simpl; auto); try solve_proper.
 
-Global Obligation Tactic := try solve_proper.
+#[export] Obligation Tactic := atomic_nonexpansive_tac.
 
 (* change start_function to handle curried arguments -- also thanks to Jason *)
 Ltac read_names term :=
@@ -840,9 +842,9 @@ Ltac start_function1 ::=
     | |- semax_body _ _ _ (_, mk_funspec _ _ _ _ ?Pre _) =>
           split3; [ check_parameter_types' | check_return_type |  ];
            match Pre with
-           | atomic_spec_pre' _ _ _ _ _ (OfeMor (rev_curry ?t)) _ _ =>
+           | atomic_spec_pre' _ _ _ _ _ (OfeMor(ofe_mor_ne := _) (rev_curry ?t)) _ _ =>
                let i := fresh in let x := read_names t in intros Espec i; destruct i as [i Q]; destruct_args x i; unfold atomic_spec_pre', atomic_spec_post', ofe_mor_car, rev_curry, tcurry; simpl tcurry_rev; cbn match (* added line *)
-           | atomic_spec_pre0 _ _ _ _ _ (OfeMor (rev_curry ?t)) _ _ =>
+           | atomic_spec_pre0 _ _ _ _ _ (OfeMor(ofe_mor_ne := _) (rev_curry ?t)) _ _ =>
                let i := fresh in let x := read_names t in intros Espec i; destruct i as [i Q]; destruct_args x i; unfold atomic_spec_pre0, atomic_spec_post0, ofe_mor_car, rev_curry, tcurry; simpl tcurry_rev; cbn match (* added line *)
            | monPred_at (convertPre _ _ (λ i, _)) =>
                intros Espec i
